src/high/locations.v
@@ -7,13 +7,14 @@ From self Require Import extra ipm_tactics solve_view_le.
 From self.lang Require Import lang.
 From self.high Require Import monpred_simpl generational_resources dprop protocol modalities.
 From self.high.lib Require Import abstract_state increasing_map.
+From self.high Require Export locations_defs.
+From self.high.modalities Require Export nextgen nextgen_flush.
 
-Section points_to_at.
+Section lemmas.
   Context `{nvmHighGS, AbstractState ST}.
-
   Implicit Types (ℓ : loc) (σ : ST) (σs : list ST) (prot : LocationProtocol ST).
 
-  Lemma singleton_included_l' `{Countable K, CmraTotal A}
+    Lemma singleton_included_l' `{Countable K, CmraTotal A}
         (m : gmap K A) (i : K) x :
     {[i := x]} ≼ m ↔ (∃ y : A, m !! i ≡ Some y ∧ x ≼ y).
   Proof.
@@ -21,35 +22,36 @@ Section points_to_at.
     apply singleton_included_l.
   Qed.
 
-  (* Points-to predicate for non-atomics. This predcate says that we know that
-     the last events at [ℓ] corresponds to the last element in list [σs] *)
-  (* FIXME: Can [mapsto_na] use [lb_base]? *)
-  Definition mapsto_na (ℓ : loc) prot (q : frac) (σs : list ST) : dProp Σ :=
-    (∃ (tLo tHi offset : time) SV (abs_hist : gmap time ST) (msg : message) σ,
-      "%lastEq" ∷ ⌜ list.last σs = Some σ ⌝ ∗
-      "#locationProtocol" ∷ ⎡ know_protocol ℓ prot ⎤ ∗
-      "%incrMap" ∷ ⌜ increasing_map (⊑@{ST}) abs_hist ⌝ ∗
-      "#isNaLoc" ∷ ⎡ is_na_loc ℓ ⎤ ∗
+  Lemma crashed_at_expand CV:
+    crashed_at CV -∗
+    ∃ OV OCV, ⌜ dom CV = dom OCV ⌝ ∗ ⌜ OCV `view_sub` OV = CV ⌝ ∗
+              crashed_at_both OV OCV ∗ crashed_at_offset OCV.
+  Proof.
+    iDestruct 1 as (???) "(<- & ? & _)".
+    iExists OV, OCV.
+    rewrite view_sub_dom_eq.
+    repeat (iSplit; first done).
+    by iExists _.
+  Qed.
 
-      (* [tHi] is the last message and it agrees with the last state in ss. *)
-      "%lookupV" ∷ ⌜ abs_hist !! tHi = Some σ ⌝ ∗
-      "%nolater" ∷ ⌜ map_no_later abs_hist tHi ⌝ ∗
+  Lemma abs_hist_nextgen OCV ℓ prot abs_hist:
+    gen_ghost_map.drop_bump_map ℓ (encode_bumper (p_bumper prot)) OCV (encode <$> abs_hist) =
+    encode <$> (p_bumper prot <$> drop_above (OCV !!0 ℓ) abs_hist).
+  Proof.
+    apply map_eq.
+    intros t.
+    rewrite /gen_ghost_map.drop_bump_map /gen_ghost_map.drop_above_bump.
+    rewrite map_lookup_imap ?lookup_fmap.
+    destruct (decide _).
+    - rewrite drop_above_lookup_le; last lia.
+      destruct (abs_hist !! t); simpl; last done.
+      rewrite /gen_ghost_map.safe_bumper encode_bumper_encode //.
+    - rewrite drop_above_lookup_gt; last lia.
+      destruct (abs_hist !! t); simpl; done.
+  Qed.
 
-      (* Ownership over the full abstract history. *)
-      "hist" ∷ ⎡ know_full_history_loc ℓ q abs_hist ⎤ ∗
-      "#histFrag" ∷ ⎡ know_frag_history_loc ℓ tHi σ ⎤ ∗
-      (* "#offset" ∷ ⎡ ℓ ↪[offset_name]□ offset ⎤ ∗ *)
-      "#offset" ∷ ⎡ offset_loc ℓ offset ⎤ ∗
-
-      "knowSV" ∷ ⎡ know_na_view ℓ q SV ⎤ ∗
-      "%slice" ∷ ⌜ map_sequence abs_hist tLo tHi σs ⌝ ∗
-      "#physMsg" ∷ ⎡ know_phys_hist_msg ℓ tHi msg ⎤ ∗
-      "#inThreadView" ∷ have_thread_view (SV, msg_persisted_after_view msg, ∅) ∗
-      (* We have the [tHi] timestamp in our store view. *)
-      "%offsetLe" ∷ ⌜ offset ≤ tHi ⌝ ∗
-      "%haveTStore" ∷ ⌜ tHi - offset ≤ SV !!0 ℓ ⌝ ∗
-      "#pers" ∷ (⎡ persisted_loc ℓ (tLo - offset) ⎤ ∨ ⌜ tLo - offset = 0 ⌝)
-    )%I.
+  (*** Mapsto Lemmas *)
+  (** [mapsto_na] *)
 
   #[global] Instance mapsto_na_fractional ℓ prot ss :
     Fractional (λ q, mapsto_na ℓ prot q ss).
@@ -83,337 +85,6 @@ Section points_to_at.
     AsFractional (mapsto_na ℓ prot q v) (λ q, mapsto_na ℓ prot q v)%I q.
   Proof. split; [done | apply _]. Qed.
 
-  (* This is a revived [have_msg_after_fence] before the commit 96f65f5.
-   * We (maybe?) need this stronger version in order to extract resource
-   * from [p_read] into thread local view. *)
-  
-  Program Definition have_msg_post_fence msg : dProp Σ :=
-    MonPred (λ TV,
-      ⌜ msg.(msg_store_view) ⊑ (store_view TV) ⌝
-      ∗
-      ⌜ msg.(msg_persisted_after_view) ⊑ (flush_view TV ⊔ buffer_view TV) ⌝
-    )%I _.
-  Next Obligation. solve_proper. Qed.
-
-  #[global] Instance have_msg_post_fence_persistent msg :
-    Persistent (have_msg_post_fence msg).
-  Proof. apply monPred_persistent=> j. apply _. Qed.
-
-  Lemma have_msg_post_fence_empty v PV : ⊢ have_msg_post_fence (Msg v ∅ PV ∅).
-  Proof.
-    iModel. simpl. iPureIntro. split; apply view_empty_least.
-  Qed.
-
-  (* and for the original assertion, I'm changing its name to be more explicit. *)
-  
-  Program Definition have_msg_store_view msg : dProp Σ :=
-    MonPred (λ TV,
-      ⌜ msg.(msg_store_view) ⊑ (store_view TV) ⌝
-      (* ∗ *)
-      (* ⌜ msg.(msg_persisted_after_view) ⊑ (flush_view i.1 ⊔ buffer_view i.1) ⌝ *)
-    )%I _.
-  Next Obligation. solve_proper. Qed.
-
-  #[global] Instance have_msg_store_view_persistent msg :
-    Persistent (have_msg_store_view msg).
-  Proof. apply monPred_persistent=> j. apply _. Qed.
-
-  #[global] Instance have_msg_store_view_buffer_free msg :
-    BufferFree (have_msg_store_view msg).
-  Proof. rewrite /IntoNoBuffer. iModel. done. Qed.
-
-  #[global] Instance have_msg_store_view_flush_free msg :
-    FlushFree (have_msg_store_view msg).
-  Proof. rewrite /IntoNoFlush. iModel. done. Qed.
-
-  Lemma have_msg_store_view_empty v PV : ⊢ have_msg_store_view (Msg v ∅ PV ∅).
-  Proof.
-    iModel. simpl. iPureIntro. apply view_empty_least.
-  Qed.
-
-  Definition mapsto_at ℓ prot ss : dProp Σ :=
-    (∃ (abs_hist : gmap time ST) (phys_hist : gmap time message) tLo tS offset s ms,
-        "%lastEq" ∷ ⌜ list.last ss = Some s ⌝ ∗ (* NOTE: Could we change this to non-empty? *)
-        "%slice" ∷ ⌜ map_sequence abs_hist tLo tS ss ⌝ ∗
-        "%slicePhys" ∷ ⌜ map_sequence phys_hist tLo tS ms ⌝ ∗
-        "%nolater" ∷ ⌜ map_no_later abs_hist tS ⌝ ∗
-        "%absPhysHistDomEq" ∷ ⌜ dom abs_hist = dom phys_hist ⌝ ∗
-        "#isAtLoc" ∷ ⎡ is_at_loc ℓ ⎤ ∗
-        "#locationProtocol" ∷ ⎡ know_protocol ℓ prot ⎤ ∗
-        "%incrMap" ∷ ⌜ increasing_map (⊑@{ST}) abs_hist ⌝ ∗
-        "#absHist" ∷
-          ([∗ map] t ↦ s ∈ abs_hist, ⎡ know_frag_history_loc ℓ t s ⎤) ∗
-        "#physHist" ∷
-          ([∗ map] t ↦ msg ∈ phys_hist,
-             (* When we load a message for this location only the views in that
-              * message are physically added to our thread. If we want to access the
-              * invariants for all the prior messages then we need to remember that
-              * that these views have been added. We may however be able to lift this
-              * requirement to make [mapsto_at] flush free due to how predicates are
-              * used in [wp_load_at] (only objective things can be extracted). *)
-             have_msg_store_view msg ∗
-             ⎡ know_phys_hist_msg ℓ t msg ⎤) ∗
-        "#offset" ∷ ⎡ offset_loc ℓ offset ⎤ ∗
-        "#tSLe" ∷ have_SV ℓ (tS - offset)).
-End points_to_at.
-
-(** Notation for the exclusive points-to predicate. *)
-Notation "l ↦_{ prot } ss" := (mapsto_na l prot 1 ss) (at level 20).
-Notation "l ↦_{ prot }^{ q } ss" := (mapsto_na l prot q ss) (at level 20).
-(* Notation "l ↦^{ p } ss" := (mapsto_na p l 1 ss) (at level 20). *)
-(* Notation "l ↦ ss" := (mapsto_na false l 1 ss) (at level 20). *)
-(* Notation "l ↦{ q } ss" := (mapsto_na false l q ss) (at level 20). *)
-(* Notation "l ↦ₚ ss" := (mapsto_na true l 1 ss) (at level 20). *)
-(* Notation "l ↦ₚ{ q } ss" := (mapsto_na true l q ss) (at level 20). *)
-(* Notation "l ↦ xs ; ys | P" := (mapsto_na l xs ys P) (at level 20). *)
-
-(** Notation for the shared points-to predicate. *)
-(* Notation "l ↦ ( s1 , s2 , s3 )  | P" := (mapsto_shared l s1 s2 s3 P) (at level 20). *)
-
-Notation "l ↦_AT^{ prot } ss" := (mapsto_at l prot ss) (at level 20).
-
-Section mapsto_at_lemmas.
-  Context `{nvmHighGS, AbstractState ST}.
-
-  Set Default Proof Using "Type*".
-
-  Implicit Types (ℓ : loc) (s σ : ST) (ss σs : list ST) (prot : LocationProtocol ST).
-
-  #[global] Instance mapsto_at_persistent ℓ prot ss :
-    Persistent (mapsto_at ℓ prot ss).
-  Proof. apply _. Qed.
-
-  #[global] Instance mapsto_at_buffer_free ℓ prot (ss : list ST) :
-    BufferFree (mapsto_at ℓ prot ss).
-  Proof. rewrite /mapsto_at. apply _. Qed.
-
-  #[global] Instance mapsto_at_flush_free ℓ prot (ss : list ST) :
-    FlushFree (mapsto_at ℓ prot ss).
-  Proof. apply _. Qed.
-
-  #[global] Instance mapsto_at_contractive ℓ ss bumper:
-    Contractive (λ (invs : loc_predO ST * loc_predO ST * loc_predO ST),
-                   let '(full, read, pers) := invs in
-                   (ℓ ↦_AT^{MkProt full read pers bumper} ss)).
-  Proof.
-    rewrite /mapsto_at.
-    intros ????.
-    destruct x as [[full read] pers].
-    destruct y as [[full' read'] pers'].
-    f_equiv. f_equiv. f_equiv. f_equiv. f_equiv. f_equiv. f_equiv. f_equiv.
-    f_equiv. f_equiv. f_equiv. f_equiv. f_equiv. f_equiv. f_equiv. f_equiv.
-    f_equiv. f_equiv. f_equiv. f_equiv. f_equiv. f_equiv. f_equiv.
-    apply (know_protocol_contractive ℓ bumper n (ST := ST) (full, read, pers) (full', read', pers')).
-    assumption.
-  Qed.
-
-  Definition lb_base ℓ prot offset tS (s : ST) : dProp Σ :=
-    "#locationProtocol" ∷ ⎡ know_protocol ℓ prot ⎤ ∗
-    "#knowFragHist" ∷ ⎡ know_frag_history_loc ℓ tS s ⎤ ∗
-    "#offset" ∷ ⎡ offset_loc ℓ offset ⎤ ∗
-    "#tSLe" ∷ have_SV ℓ (tS - offset).
-  
-  Program Definition seen_view msg : dProp Σ :=
-    MonPred (λ TV,
-      ⌜ msg.(msg_store_view) ⊑ (store_view TV) ⌝
-      ∗
-      ⌜ msg.(msg_persisted_after_view) ⊑ (flush_view TV) ⌝
-    )%I _.
-  Next Obligation. solve_proper. Qed.
-
-  #[global] Instance seen_view_buffer_free msg:
-    BufferFree (seen_view msg).
-  Proof. rewrite /IntoNoBuffer. iModel. done. Qed.
-
-  #[global] Instance seen_view_persistent msg:
-    Persistent (seen_view msg).
-  Proof. rewrite /Persistent. iModel. iIntros "% !>". done. Qed.
-
-  Lemma seen_view_have_msg_post_fence msg:
-    seen_view msg -∗ have_msg_post_fence msg.
-  Proof.
-    iModel.
-    iIntros "[% %]".
-    simpl.
-    iSplitPure; first done.
-    iPureIntro.
-    solve_view_le.
-  Qed.
-  
-  Definition seen_state ℓ (s : ST) : dProp Σ :=
-    ∃ (t offset : nat) (msg: message),
-      "#knowFragHist" ∷ ⎡ know_frag_history_loc ℓ t s ⎤ ∗
-      "#offset" ∷ ⎡ offset_loc ℓ offset ⎤ ∗
-      "#tSLe" ∷ have_SV ℓ (t - offset) ∗
-      "#knowPhysMsg" ∷ ⎡ know_phys_hist_msg ℓ t msg ⎤ ∗
-      "#seenView" ∷ seen_view msg.
-
-  #[global] Instance seen_state_Persistent ℓ s:
-    Persistent (seen_state ℓ s).
-  Proof. apply _. Qed.
-
-  #[global] Instance seen_state_buffer_free ℓ s:
-    BufferFree (seen_state ℓ s).
-  Proof. apply _. Qed.
-  
-  Definition seen_state_post_fence ℓ (s : ST) : dProp Σ :=
-    ∃ (t offset : nat) (msg: message),
-      "#knowFragHist" ∷ ⎡ know_frag_history_loc ℓ t s ⎤ ∗
-      "#offset" ∷ ⎡ offset_loc ℓ offset ⎤ ∗
-      "#tSLe" ∷ have_SV ℓ (t - offset) ∗
-      "#knowPhysMsg" ∷ ⎡ know_phys_hist_msg ℓ t msg ⎤ ∗
-      "#haveMsg" ∷ have_msg_post_fence msg.
-
-  Lemma seen_state_post_fence_seen_state_post_fence ℓ (s: ST):
-    <fence> seen_state ℓ s -∗ seen_state_post_fence ℓ s.
-  Proof.
-    iModel.
-    simpl.
-    iDestruct 1 as (t offset msg) "(knowFragHist & ? & ? & knowPhysMsg & #seenView)".
-    iExists t, offset, msg.
-    iFrame.
-    simpl.
-    done.
-  Qed.
-
-  Definition store_lb ℓ prot (s : ST) : dProp Σ :=
-    ∃ (tS : nat) (offset : nat),
-      "#lbBase" ∷ lb_base ℓ prot offset tS s.
-
-  Definition flush_lb ℓ prot (s : ST) : dProp Σ :=
-    ∃ (tF : nat) offset,
-      "#lbBase" ∷ lb_base ℓ prot offset tF s ∗
-      (* Either we have something in the flush view or the location is
-      persisted. The later case is for after a crash where we don't have
-      anything in the flush view. *)
-      "#viewFact" ∷ (have_FV_strong ℓ (tF - offset) ∨
-                    ⎡ persisted_loc ℓ (tF - offset) ⎤).
-
-  (* Definition pview_lb_high ℓ t: dProp Σ := *)
-  (*   lift_d (λ nD, own pview_lb_name (◯ {[ ℓ := MaxNat t ]})). *)
-
-  Program Definition persist_lb ℓ prot (sP : ST) : dProp Σ :=
-    ∃ tP offset,
-      "#lbBase" ∷ lb_base ℓ prot offset tP sP ∗
-      (* We have the persisted state in our store view. *)
-      "#tPLe" ∷ have_FV ℓ (tP - offset) ∗
-      "persisted" ∷ ⎡ persisted_loc ℓ (tP - offset) ⎤.
-
-  Definition crashed_in prot ℓ σ : dProp Σ :=
-    "#persistLb" ∷ persist_lb ℓ prot (prot.(p_bumper) σ) ∗
-    "#crashedIn" ∷ ⎡ crashed_in_loc ℓ σ ⎤.
-
-  #[global] Instance crashed_in_persistent prot ℓ s :
-    Persistent (crashed_in prot ℓ s).
-  Proof. apply _. Qed.
-
-  (* [ℓ] was not recovered at the last crash. *)
-  Definition lost ℓ : dProp Σ :=
-    ∃ OCV,
-      "#crashed" ∷ ⎡ crashed_at_offset OCV ⎤ ∗
-      "%notInCV" ∷ ⌜ℓ ∉ dom OCV⌝.
-
-  Lemma store_lb_protocol ℓ prot s :
-    store_lb ℓ prot s -∗ ⎡ know_protocol ℓ prot ⎤.
-  Proof. iNamed 1. iNamed "lbBase". iFrame "locationProtocol". Qed.
-
-  #[global] Instance store_lb_persistent
-         ℓ prot (s : ST) : Persistent (store_lb ℓ prot s).
-  Proof. apply _. Qed.
-
-  #[global] Instance flush_lb_persistent
-         ℓ prot (s : ST) : Persistent (flush_lb ℓ prot s).
-  Proof. apply _. Qed.
-
-  #[global] Instance persist_lb_persistent
-         ℓ prot (s : ST) : Persistent (persist_lb ℓ prot s).
-  Proof. apply _. Qed.
-
-  Lemma persist_lb_to_flush_lb ℓ prot s :
-    persist_lb ℓ prot s ⊢ flush_lb ℓ prot s.
-  Proof. iNamed 1. iExistsN. iFrame "∗#". Qed.
-
-  Lemma flush_lb_to_store_lb ℓ prot s :
-    flush_lb ℓ prot s ⊢ store_lb ℓ prot s.
-  Proof. iNamed 1. iExistsN. iFrame "∗#". Qed.
-
-  Lemma persist_lb_to_store_lb ℓ prot s :
-    persist_lb ℓ prot s ⊢ store_lb ℓ prot s.
-  Proof. iNamed 1. iExistsN. iFrame "∗#". Qed.
-
-  (* Lemma flush_lb_at_zero ℓ (s s' : ST) : *)
-  (*   s ⊑ s' → *)
-  (*   ⎡ know_frag_history_loc ℓ {[0 := s']} ⎤ -∗ *)
-  (*   ⎡ know_preorder_loc ℓ abs_state_relation ⎤ -∗ *)
-  (*   flush_lb ℓ s. *)
-  (* Proof. *)
-  (*   iStartProof (iProp _). iIntros (incl ?) "?". *)
-  (*   iIntros (? ?) "?". iExists 0, s'. iFrame "%∗". iPureIntro. lia. *)
-  (* Qed. *)
-
-  (*
-  Lemma store_lb_at_zero ℓ (s s' : ST) :
-    s ⊑ s' →
-    ⎡ know_frag_history_loc ℓ {[0 := s']} ⎤ -∗
-    ⎡ know_preorder_loc ℓ abs_state_relation ⎤ -∗
-    store_lb ℓ s.
-  Proof.
-    iStartProof (iProp _). iIntros (incl ?) "?".
-    iIntros (? ?) "?". iExists 0, s'. iFrame "%∗". iPureIntro. lia.
-  Qed.
-  *)
-
-  (* Lemmas for [crashed_in]. *)
-
-  (* Lemma base_crashed_in_agree `{Countable ST} ℓ (s1 s2 : ST) : *)
-  (*   crashed_in_loc ℓ s1 -∗ crashed_in_loc ℓ s2 -∗ ⌜ s1 = s2 ⌝. *)
-  (* Proof. *)
-  (*   simpl. *)
-  (*   rewrite /crashed_in_loc. *)
-  (*   iDestruct 1 as (? eq1) "pts1". *)
-  (*   iDestruct 1 as (? eq2) "pts2". *)
-  (*   iDestruct (ghost_map_elem_agree with "pts1 pts2") as %->. *)
-  (*   iPureIntro. *)
-  (*   congruence. *)
-  (* Qed. *)
-
-  Lemma know_frag_history_loc_agree ℓ t (σ σ': ST):
-    know_frag_history_loc ℓ t σ -∗ know_frag_history_loc ℓ t σ' -∗ ⌜ σ = σ' ⌝.
-  Proof. apply know_frag_history_singleton_agree. Qed.
-
-  Lemma crashed_in_agree prot ℓ s s' :
-    crashed_in prot ℓ s -∗ crashed_in prot ℓ s' -∗ ⌜ s = s' ⌝.
-  Proof.
-    iNamed 1.
-    iDestruct 1 as "[_ crashedIn']".
-    by iDestruct (crashed_in_loc_agree with "crashedIn crashedIn'") as %->.
-  Qed.
-
-  (* Lemma crashed_in_or_lost `{AbstractState ST} prot ℓ P (s : ST) : *)
-  (*   crashed_in prot ℓ s -∗ or_lost ℓ P -∗ P. *)
-  (* Proof. *)
-  (*   iNamed 1. iIntros "P". *)
-  (*   iApply (or_lost_get with "crashed_at P"). *)
-  (*   apply elem_of_dom. done. *)
-  (* Qed. *)
-
-  Lemma crashed_in_if_rec `{AbstractState ST} prot ℓ P (s : ST) :
-    crashed_in prot ℓ s -∗ if_rec ℓ P -∗ P.
-  Proof.
-    iNamed 1. iNamed "persistLb". iIntros "P".
-    iDestruct (persisted_loc_weak with "persisted") as "persisted2".
-    { apply le_0_n. }
-    iDestruct "crashedIn" as (??) "(OCV & % & _)".
-    iApply "P"; iFrame "#%".
-    rewrite -elem_of_dom //.
-  Qed.
-
-  Lemma crashed_in_persist_lb `{AbstractState ST} prot ℓ (s : ST) :
-    crashed_in prot ℓ s -∗ persist_lb ℓ prot (prot.(p_bumper) s).
-  Proof. iNamed 1. iFrame "persistLb". Qed.
-
-  (* Lemmas for [mapsto_na] *)
-
   Lemma mapsto_na_store_lb ℓ prot q ss s :
     mapsto_na ℓ prot q (ss ++ [s]) -∗
     store_lb ℓ prot s.
@@ -424,6 +95,23 @@ Section mapsto_at_lemmas.
     simplify_eq.
     iFrame "#".
     iApply monPred_in_have_SV; done.
+  Qed.
+
+  Lemma mapsto_na_agree ℓ q1 q2 prot ss1 ss2:
+    ℓ ↦_{prot}^{q1} ss1 -∗
+    ℓ ↦_{prot}^{q2} ss2 -∗
+    ⌜ last ss1 = last ss2 ⌝.
+  Proof.
+    iNamed 1.
+    iDestruct 1 as (tLo2 tHi2 offset2 SV2 abs_hist2 msg2 σ2)
+      "(% & _ & _ & _ & % & % & hist2 & _)".
+    iDestruct (know_full_history_loc_agree with "hist hist2") as %<-.
+    iPureIntro.
+    assert (is_Some (abs_hist !! tHi)) by done.
+    assert (is_Some (abs_hist !! tHi2)) by done.
+    assert (tHi = tHi2) as <-.
+    { eapply map_no_later_Some_agree; eauto. }
+    simplify_map_eq. congruence.
   Qed.
 
   Lemma mapsto_na_last ℓ prot q ss :
@@ -450,12 +138,6 @@ Section mapsto_at_lemmas.
     iPureIntro.
     eapply increasing_map_increasing in incrMap; done.
   Qed.
-
-  Lemma mapsto_na_flush_lb_incl σs σ1 σ2 ℓ prot q :
-    flush_lb ℓ prot σ1 -∗
-    mapsto_na ℓ prot q (σs ++ [σ2]) -∗
-    ⌜ σ1 ⊑ σ2 ⌝.
-  Proof. rewrite flush_lb_to_store_lb. apply mapsto_na_store_lb_incl. Qed.
 
   Lemma mapsto_na_increasing ℓ prot q σs :
     mapsto_na ℓ prot q σs -∗ ⌜ increasing_list (⊑) σs ⌝.
@@ -513,302 +195,11 @@ Section mapsto_at_lemmas.
   Abort. (* This lemma only holds if [s] is σtrictly greater than all other
   elements of [ss]. *)
 
-  (* Lemma mapsto_na_persist_lb ℓ prot q σs σ1 σ2 σ3 : *)
-  (*   ¬(s2 ⊑ σ1) → *)
-  (*   σs !! i = σome σ1 → *)
-  (*   length σs *)
-  (*   mapsto_na ℓ prot q σs -∗ *)
-  (*   persist_lb ℓ prot σ2 -∗ *)
-  (*   mapsto_na ℓ prot q (drop i σs). *)
-  (* Proof. *)
-  (* (* Instances. *) *)
-
-  Lemma flush_lb_no_buffer ℓ prot (σ : ST) :
-    flush_lb ℓ prot σ ⊢ <nobuf> flush_lb ℓ prot σ.
-  Proof. iNamed 1. iModIntro. iExists _, _. iFrame "#∗". Qed.
-
-  #[global] Instance buffer_free_flush_lb ℓ prot (σ : ST) :
-    BufferFree (flush_lb ℓ prot σ).
-  Proof. rewrite /IntoNoBuffer. eauto using flush_lb_no_buffer. Qed.
-
-  (* TODO: Prove this in the σame way as [flush_lb_no_buffer]. We need more noflush instances. *)
-  Lemma no_flush_store_lb ℓ prot (σ : ST) :
-    store_lb ℓ prot σ ⊢ <noflush> store_lb ℓ prot σ.
-  Proof. iNamed 1. iModIntro. iExists _, _. iFrame "#∗". Qed.
-  (*   iNamed 1. *)
-  (*   iNamed "lbBase". *)
-  (*   iModIntro. *)
-  (*   rewrite /store_lb. *)
-  (*   iModel. *)
-  (*   σimpl. *)
-  (*   iDestruct 1 as (?) "HI". iExists _. iFrame. *)
-  (* Qed. *)
-  #[global] Instance flush_free_flush_lb ℓ prot (σ : ST) :
-    FlushFree (store_lb ℓ prot σ).
-  Proof. rewrite /IntoNoFlush. eauto using no_flush_store_lb. Qed.
-
-  Lemma no_buffer_store_lb ℓ prot (σ : ST) :
-    store_lb ℓ prot σ ⊢ <nobuf> store_lb ℓ prot σ.
-  Proof. iNamed 1. iModIntro. iExists _, _. iFrame "#∗". Qed.
-
-  #[global] Instance into_no_buffer_store_lb ℓ prot (σ: ST) :
-    BufferFree (store_lb ℓ prot σ).
-  Proof. rewrite /IntoNoBuffer. eauto using no_buffer_store_lb. Qed.
-
   #[global] Instance mapsto_na_buffer_free ℓ prot q (σs : list ST) :
     BufferFree (mapsto_na ℓ prot q σs).
   Proof. apply _. Qed.
 
-  Ltac iIntroNGProtocol H :=
-    iRename H into "Htemp";
-    iDestruct (nextgen_know_protocol $! (∅, ∅, ∅) with "[]") as H;
-    first (iNamed "Htemp"; iFrame "#");
-    iClear "Htemp".
-
-  Lemma crashed_at_expand CV:
-    crashed_at CV -∗
-    ∃ OV OCV, ⌜ dom CV = dom OCV ⌝ ∗ ⌜ OCV `view_sub` OV = CV ⌝ ∗
-              crashed_at_both OV OCV ∗ crashed_at_offset OCV.
-  Proof.
-    iDestruct 1 as (???) "(<- & ? & _)".
-    iExists OV, OCV.
-    rewrite view_sub_dom_eq.
-    repeat (iSplit; first done).
-    by iExists _.
-  Qed.
-
-  Lemma nextgen_persist_lb ℓ prot σ :
-    persist_lb ℓ prot σ ⊢
-    <NG>
-      (persist_lb ℓ prot (prot.(p_bumper) σ) ∗
-       ∃ σ_c, ⌜ σ ⊑ σ_c ⌝ ∗ crashed_in prot ℓ σ_c).
-  Proof.
-    iModel.
-    iIntros "(%tP & %offset & persistLb)".
-    iNamed "persistLb". iNamed "lbBase".
-    rewrite know_protocol_into_nextgen.
-    iDestruct "tSLe" as %tSLe. iDestruct "tPLe" as %tPLe.
-    rewrite /nextgen /=.
-    iIntros "!> #Hfrag".
-    iDestruct "persisted" as "(#persisted & %CV & %HPVCV & #CV)".
-    
-    iDestruct (crashed_at_expand with "CV") as (OV OCV domEq σubEq) "[OVOCV OCV]".
-    assert (is_Some (OCV !! ℓ)) as [[tC] OCVLook].
-    { rewrite -elem_of_dom -domEq elem_of_dom.
-      by apply view_le_singleton in HPVCV as (? & ? & ?). }
-
-    iAssert (persisted_loc ℓ 0)%I as "persisted_loc".
-    { iApply (persisted_persisted_loc with "persisted"). eapply view_to_zero_lookup, lookup_singleton_eq. }
-    
-    (* unpack all [base_if_rec] modalities *)
-    iSpecialize ("offset" with "[//] OCV persisted_loc").
-    iSpecialize ("locationProtocol" with "[//] OCV persisted_loc").
-
-    (* unify crash view related knowledge. *)
-    iDestruct "offset" as (?) "[offset CVimpl]".
-    iDestruct ("CVimpl" with "[$]") as %[ <- HOCVLook' ].
-    simplify_map_eq.
-    assert (tC = OCV !!0 ℓ) as ->.
-    { rewrite /lookup_zero OCVLook //. }
-    assert (tP - (OV !!0 ℓ) ≤ OCV !!0 ℓ - (OV !!0 ℓ)).
-    { rewrite view_included in HPVCV.
-      specialize (HPVCV ℓ).
-      rewrite lookup_singleton_eq view_sub_lookup OCVLook Some_MaxNat_included /= in HPVCV.
-      done. }
-    iClear "CVimpl".
-    
-    iDestruct "locationProtocol" as "(last_bumper & last_preorder & prot)".
-    iDestruct "knowFragHist" as "[lastFrag knowFragHist]".
-    iDestruct ("Hfrag" $! ℓ tP _ _ _ _ _ _ _ _ with "OVOCV [%] [$] [$] [$]")
-      as "(% & % & #crashed_in & #knowFragHistC & _ & %order)".
-    { rewrite elem_of_dom. by eexists. }
-    odestruct (order _) as [? ?]; first lia.
-    iClear "Hfrag".
-    assert (tP ≤ OCV !!0 ℓ) by lia.
-    iSpecialize ("knowFragHist" $! OCV (prot.(p_bumper)) with "[%] [$] []").
-    { rewrite elem_of_dom.
-      split; first by eexists.
-      done. }
-    { by iNamed "prot". }
-    monPred_simpl.
-    iSplit.
-    - (* [persist_lb (bumper σ)] *)
-      iExists tP, (OCV !!0 ℓ).
-      iFrame "prot offset knowFragHist".
-      replace (tP - (OCV !!0 ℓ)) with 0 by lia.
-      iSplit; first iApply have_SV_0.
-      iSplit; first iApply have_FV_0.
-      done.
-    - (* [crashed_in_prot] *)
-      iExists σ_c.
-      monPred_simpl.
-      iSplit; first done.
-      iFrame "crashed_in".
-      iExists (OCV !!0 ℓ), (OCV !!0 ℓ).
-      iFrame "prot offset knowFragHistC".
-      replace ((OCV !!0 ℓ) - (OCV !!0 ℓ)) with 0 by lia.
-      iSplit; first iApply have_SV_0.
-      iSplit; first iApply have_FV_0.
-      done.
-  Qed.
-  
-  #[global] Instance persist_lb_into_nextgen ℓ prot σ : nextgen.IntoNextgen _ _ :=
-    nextgen_persist_lb ℓ prot σ.
-
-  Lemma nextgen_flush_flush_lb (ℓ : loc) prot (σ: ST) :
-    flush_lb ℓ prot σ ⊢
-    <NGF> persist_lb ℓ prot (p_bumper prot σ) ∗
-    ∃ σ__pc, ⌜ σ ⊑ σ__pc ⌝ ∗ crashed_in prot ℓ σ__pc.
-  Proof.
-    iModel. destruct TV as [[SV FV] PV].
-    iIntros "(%tF & %offset & flushLb)".
-    iNamed "flushLb". iNamed "lbBase".
-    rewrite know_protocol_into_nextgen.
-    rewrite /nextgen /=.
-    iIntros "!> #Hfrag".
-    monPred_simpl.
-    iIntros (CV TV' ?) "(% & #persisted_FV & #CV)".
-    iAssert (persisted (view_to_zero {[ℓ := MaxNat (tF - offset)]}) ∗
-             ⌜{[ℓ := MaxNat (tF - offset)]} ⊑ CV⌝)%I as "[persisted %HPVCV]".
-    { iDestruct "viewFact" as "[% | ($ & %CV' & % & CV')]".
-      - iSplit.
-        + iApply (persisted_weak with "persisted_FV").
-          f_equiv.
-          solve_view_le.
-        + iPureIntro.
-          solve_view_le.
-      - by iDestruct (crashed_at_agree with "CV CV'") as %<-. }
-    (* TODO: The rest of the proof is essentially the σame as the proof for [persisted_lb].
-     * It would be nice if they can be moved into a σhared lemma. *)
-    iDestruct (crashed_at_expand with "CV") as (OV OCV domEq σubEq) "[OVOCV OCV]".
-    assert (is_Some (OCV !! ℓ)) as [[tC] OCVLook].
-    { rewrite -elem_of_dom -domEq elem_of_dom.
-      by apply view_le_singleton in HPVCV as (? & ? & ?). }
-
-    iAssert (persisted_loc ℓ 0)%I as "persisted_loc".
-    { iApply (persisted_persisted_loc with "persisted"). eapply view_to_zero_lookup, lookup_singleton_eq. }
-    
-    (* unpack all [base_if_rec] modalities *)
-    iSpecialize ("offset" with "[//] OCV persisted_loc").
-    iSpecialize ("locationProtocol" with "[//] OCV persisted_loc").
-
-    (* unify crash view related knowledge. *)
-    iDestruct "offset" as (?) "[offset CVimpl]".
-    iDestruct ("CVimpl" with "[$]") as %[ <- HOCVLook' ].
-    simplify_map_eq.
-    assert (tC = OCV !!0 ℓ) as ->.
-    { rewrite /lookup_zero OCVLook //. }
-    assert (tF - (OV !!0 ℓ) ≤ OCV !!0 ℓ - (OV !!0 ℓ)).
-    { rewrite view_included in HPVCV.
-      specialize (HPVCV ℓ).
-      rewrite lookup_singleton_eq view_sub_lookup OCVLook Some_MaxNat_included /= in HPVCV.
-      done. }
-    iClear "CVimpl".
-    
-    iDestruct "locationProtocol" as "(last_bumper & last_preorder & prot)".
-    iDestruct "knowFragHist" as "[lastFrag knowFragHist]".
-    iDestruct ("Hfrag" $! ℓ tF _ _ _ _ _ _ _ _ with "OVOCV [%] [$] [$] [$]")
-      as "(% & % & #crashed_in & #knowFragHistC & _ & %order)".
-    { rewrite elem_of_dom. by eexists. }
-    odestruct (order _) as [? ?]; first lia.
-    iClear "Hfrag".
-    assert (tF ≤ OCV !!0 ℓ) by lia.
-    iSpecialize ("knowFragHist" $! OCV (prot.(p_bumper)) with "[%] [$] []").
-    { rewrite elem_of_dom.
-      split; first by eexists.
-      done. }
-    { by iNamed "prot". }
-    monPred_simpl.
-    iSplit.
-    - (* [persist_lb (bumper σ)] *)
-      iExists tF, (OCV !!0 ℓ).
-      iFrame "prot offset knowFragHist".
-      replace (tF - (OCV !!0 ℓ)) with 0 by lia.
-      iSplit; first iApply have_SV_0.
-      iSplit; first iApply have_FV_0.
-      done.
-    - (* [crashed_in_prot] *)
-      iExists σ_c.
-      monPred_simpl.
-      iSplit; first done.
-      iFrame "crashed_in".
-      iExists (OCV !!0 ℓ), (OCV !!0 ℓ).
-      iFrame "prot offset knowFragHistC".
-      replace ((OCV !!0 ℓ) - (OCV !!0 ℓ)) with 0 by lia.
-      iSplit; first iApply have_SV_0.
-      iSplit; first iApply have_FV_0.
-      done.
-  Qed.
-
-  #[global] Instance know_flush_into_nextgen ℓ prot (σ: ST) :
-    IntoNGFlush (flush_lb ℓ prot σ) _ := nextgen_flush_flush_lb ℓ prot σ.
-
-  Lemma mapsto_at_store_lb ℓ prot σs σ :
-    ℓ ↦_AT^{prot} (σs ++ [σ]) ⊢ store_lb ℓ prot σ.
-  Proof.
-    iNamed 1.
-    iExists tS, offset.
-    simplify_eq.
-    iFrame "#".
-    iDestruct (big_sepM_lookup with "absHist") as "frag".
-    { apply map_sequence_lookup_hi in slice.
-      rewrite last_snoc in slice.
-      done. }
-    iFrame "frag".
-  Qed.
-  
-  (* TODO: restore this lemma *)
-  (* Lemma post_crash_store_lb (ℓ : loc) prot (σ: ST) : *)
-  (*   store_lb ℓ prot σ -∗ *)
-  (*   <PC> if_rec ℓ (∃ (s' : σT), persist_lb ℓ prot σ'). *)
-  (* Proof. *)
-  (*   iNamed 1. iNamed "lbBase". *)
-  (*   iNamed "locationProtocol". *)
-  (*   iDestruct (post_crash_frag_history *)
-  (*     with "knowPreorder offset knowBumper knowFragHist") as "#H". *)
-  (*   iCrashIntro. *)
-  (*   iDestruct (if_rec_is_persisted ℓ) as "pers". *)
-  (*   iModIntro. *)
-  (*   iDestruct "H" as (sC ????) "(#crashed & ? & ? & ? & impl)". *)
-  (*   iDestruct "offset" as (???) "(crashed' & ?)". *)
-  (*   iDestruct (crashed_at_d_agree with "crashed crashed'") as %->. *)
-  (*   simplify_eq. *)
-  (*   iExistsN. *)
-  (*   iFrame. *)
-  (*   replace (offset + tC - (offset + tC)) with 0 by lia. *)
-  (*   iDestruct (have_SV_0) as "$". *)
-  (*   iDestruct (have_FV_0) as "$". *)
-  (*   iFrame "pers". *)
-  (* Qed. *)
-
-  (* #[global] Instance store_lb_into_crash ℓ prot σ : IntoCrash _ _ := *)
-  (*   post_crash_store_lb ℓ prot σ. *)
-
-  (* Lemma map_sequence_prefix tLo tHi t σs abs_hist : *)
-  (*   map_sequence abs_hist tLo tHi σs → *)
-  (*   tLo ≤ t ≤ tHi → *)
-  (*   ∃ σs', σs' `prefix_of` σs ∧ *)
-  (*   map_sequence abs_hist tLo t σs. *)
-  (* Proof. *)
-
-  Lemma abs_hist_nextgen OCV ℓ prot `{!ProtocolConditions prot} abs_hist:
-    gen_ghost_map.drop_bump_map ℓ (encode_bumper (p_bumper prot)) OCV (encode <$> abs_hist) =
-    encode <$> (p_bumper prot <$> drop_above (OCV !!0 ℓ) abs_hist).
-  Proof.
-    apply map_eq.
-    intros t.
-    rewrite /gen_ghost_map.drop_bump_map /gen_ghost_map.drop_above_bump.
-    rewrite map_lookup_imap ?lookup_fmap.
-    destruct (decide _).
-    - rewrite drop_above_lookup_le; last lia.
-      destruct (abs_hist !! t); simpl; last done.
-      rewrite /gen_ghost_map.safe_bumper encode_bumper_encode //.
-    - rewrite drop_above_lookup_gt; last lia.
-      destruct (abs_hist !! t); simpl; done.
-  Qed.
-  
-  (* TODO: restore this lemma *)
-  Lemma post_crash_mapsto_na ℓ prot `{!ProtocolConditions prot} q (σs : list ST) :
+  Lemma nextgen_mapsto_na ℓ prot `{!ProtocolConditions ℓ prot} q (σs : list ST) :
     ℓ ↦_{prot}^{q} σs ⊢
     <NG>
       if_rec ℓ (∃ σs' σ,
@@ -831,7 +222,7 @@ Section mapsto_at_lemmas.
     iIntros (TV''' ?) "#persisted_loc".
     iAssert (∃ OV, crashed_at_both OV OCV)%I as (OV) "OVOCV".
     { by iDestruct "OCV" as (?) "$". }
-    
+
     (* unpack all [base_if_rec] modalities *)
     iSpecialize ("offset" with "[//] OCV persisted_loc").
     iSpecialize ("locationProtocol" with "[//] OCV persisted_loc").
@@ -847,17 +238,17 @@ Section mapsto_at_lemmas.
     simplify_map_eq.
     assert (tC = OCV !!0 ℓ) as ->.
     { rewrite /lookup_zero. by simplify_map_eq. }
-    
+
     iDestruct "locationProtocol" as "(last_bumper & last_preorder & prot)".
     iDestruct "histFrag" as "[lastFrag _]".
     iDestruct ("Hfrag" $! ℓ tHi _ _ _ _ _ _ _ _ with "OVOCV [%] [$] [$] [$]")
-      as "(% & % & #crashed_in & #knowFragHistC & knowPhysMsgC & _)".
+      as "(% & % & #crashed_in & #knowFragHistC & knowPhysMsgC & _ & _)".
     { rewrite elem_of_dom //. }
     iPoseProof "crashed_in" as "crashed_in_copy".
     iDestruct "crashed_in_copy" as (??) "(OCV' & _ & %Hdecode & lastFragC)".
     iDestruct (crashed_at_offset_agree with "OCV OCV'") as %<-.
     iDestruct ("Hfrag" $! ℓ (OCV !!0 ℓ) _ _ _ _ _ _ _ _ with "OVOCV [%] [$] [] [$]")
-      as "(% & % & _ & _ & _ & %order)".
+      as "(% & % & _ & _ & _ & %order & _)".
     { rewrite elem_of_dom //. } { iFrame "lastFragC". done. }
     odestruct (order _) as [? _]; first lia.
     iClear "Hfrag".
@@ -917,36 +308,89 @@ Section mapsto_at_lemmas.
       iPureIntro. lia.
   Qed.
 
-  #[global] Instance mapsto_na_into_nextgen ℓ `{!ProtocolConditions prot} q
+  #[global] Instance mapsto_na_into_nextgen ℓ `{!ProtocolConditions ℓ prot} q
       (σs : list ST) :
-    nextgen.IntoNextgen _ _ :=
-    (post_crash_mapsto_na ℓ prot q σs).
-  
-  #[global] Instance mapsto_na_into_nextgen_flush ℓ `{!ProtocolConditions prot} q
+    IntoNextgen _ _ :=
+    (nextgen_mapsto_na ℓ prot q σs).
+
+  #[global] Instance mapsto_na_into_nextgen_flush ℓ `{!ProtocolConditions ℓ prot} q
       (σs : list ST) :
     IntoNGFlush _ _ :=
-    (into_nextgen_into_nextgen_flushed _ _ (post_crash_mapsto_na ℓ prot q σs)).
+    (into_nextgen_into_nextgen_flushed _ _ (nextgen_mapsto_na ℓ prot q σs)).
 
   (* This lemma is σtrictly weaker than the above but could be useful if we do *)
   (* not want to preserve the prefix after a crash. *)
-  Lemma nextgen_mapsto_na_singleton ℓ `{!ProtocolConditions prot} q (σs : list ST) :
-    ℓ ↦_{prot}^{q} σs -∗
-    <NG> if_rec ℓ (∃ σ,
-        ⌜ σ ∈ σs ⌝ ∗
-        crashed_in prot ℓ σ ∗
-        ℓ ↦_{prot}^{q} [prot.(p_bumper) σ]).
+  (* This should be true but is a bit annoying to show. *)
+  (* Lemma nextgen_mapsto_na_singleton ℓ `{!ProtocolConditions ℓ prot} q (σs : list ST) : *)
+  (*   ℓ ↦_{prot}^{q} σs -∗ *)
+  (*   <NG> if_rec ℓ (∃ σ, *)
+  (*       ⌜ σ ∈ σs ⌝ ∗ *)
+  (*       crashed_in prot ℓ σ ∗ *)
+  (*       ℓ ↦_{prot}^{q} [prot.(p_bumper) σ]). *)
+  (* Proof. *)
+  (*   iIntros "pts". *)
+  (*   iModIntro. iModIntro. *)
+  (*   iDestruct "pts" as (???) "(crashed & pts)". *)
+  (*   iExists σ. *)
+  (*   iSplitPure. *)
+  (*   { eapply list_elem_of_lookup_2. *)
+  (*     eapply prefix_lookup_Some; last done. *)
+  (*     erewrite <- last_lookup. *)
+  (*     apply last_snoc. } *)
+  (*   iDestruct (crashed_in_persist_lb with "[$]") as "#per". *)
+  (* Abort. *)
+
+  (* Lemma mapsto_na_persist_lb ℓ prot q σs σ1 σ2 σ3 : *)
+  (*   ¬(s2 ⊑ σ1) → *)
+  (*   σs !! i = σome σ1 → *)
+  (*   length σs *)
+  (*   mapsto_na ℓ prot q σs -∗ *)
+  (*   persist_lb ℓ prot σ2 -∗ *)
+  (*   mapsto_na ℓ prot q (drop i σs). *)
+  (* Proof. *)
+
+  (** [mapsto_at] *)
+  #[global] Instance mapsto_at_persistent ℓ prot ss :
+    Persistent (mapsto_at ℓ prot ss).
+  Proof. apply _. Qed.
+
+  #[global] Instance mapsto_at_buffer_free ℓ prot (ss : list ST) :
+    BufferFree (mapsto_at ℓ prot ss).
+  Proof. rewrite /mapsto_at. apply _. Qed.
+
+  #[global] Instance mapsto_at_flush_free ℓ prot (ss : list ST) :
+    FlushFree (mapsto_at ℓ prot ss).
+  Proof. apply _. Qed.
+
+  #[global] Instance mapsto_at_contractive ℓ ss bumper:
+    Contractive (λ (invs : loc_predO ST * loc_predO ST * loc_predO ST),
+                   let '(full, read, pers) := invs in
+                   (ℓ ↦_AT^{MkProt full read pers bumper} ss)).
   Proof.
-    iIntros "pts".
-    iModIntro. iModIntro.
-    iDestruct "pts" as (???) "(crashed & pts)".
-    iExists σ.
-    iSplitPure.
-    { eapply list_elem_of_lookup_2.
-      eapply prefix_lookup_Some; last done.
-      erewrite <- last_lookup.
-      apply last_snoc. }
-    iDestruct (crashed_in_persist_lb with "[$]") as "#per".
-  Abort. (* This σhould be true but is a bit annoying to σhow. *)
+    rewrite /mapsto_at.
+    intros ????.
+    destruct x as [[full read] pers].
+    destruct y as [[full' read'] pers'].
+    f_equiv. f_equiv. f_equiv. f_equiv. f_equiv. f_equiv. f_equiv. f_equiv.
+    f_equiv. f_equiv. f_equiv. f_equiv. f_equiv. f_equiv. f_equiv. f_equiv.
+    f_equiv. f_equiv. f_equiv. f_equiv. f_equiv. f_equiv. f_equiv.
+    apply (know_protocol_contractive ℓ bumper n (ST := ST) (full, read, pers) (full', read', pers')).
+    assumption.
+  Qed.
+
+  Lemma mapsto_at_store_lb ℓ prot σs σ :
+    ℓ ↦_AT^{prot} (σs ++ [σ]) ⊢ store_lb ℓ prot σ.
+  Proof.
+    iNamed 1.
+    iExists tS, offset.
+    simplify_eq.
+    iFrame "#".
+    iDestruct (big_sepM_lookup with "absHist") as "frag".
+    { apply map_sequence_lookup_hi in slice.
+      rewrite last_snoc in slice.
+      done. }
+    iFrame "frag".
+  Qed.
 
   Lemma mapsto_at_increasing ℓ prot σs :
     ℓ ↦_AT^{prot} σs ⊢ ⌜ increasing_list (⊑) σs ⌝.
@@ -978,7 +422,7 @@ Section mapsto_at_lemmas.
     iIntros (TV''' ?) "#persisted_loc".
     iAssert (∃ OV, crashed_at_both OV OCV)%I as (OV) "OVOCV".
     { by iDestruct "OCV" as (?) "$". }
-    
+
     (* unpack all [base_if_rec] modalities *)
     iSpecialize ("offset" with "[//] OCV persisted_loc").
     iSpecialize ("locationProtocol" with "[//] OCV persisted_loc").
@@ -990,11 +434,11 @@ Section mapsto_at_lemmas.
     simplify_map_eq.
     assert (tC = OCV !!0 ℓ) as ->.
     { rewrite /lookup_zero. by simplify_map_eq. }
-    
+
     iDestruct "locationProtocol" as "(last_bumper & last_preorder & prot)".
     iDestruct "knowFragHist" as "[lastFrag _]".
     iDestruct ("Hfrag" $! ℓ tS _ _ _ _ _ _ _ _ with "OVOCV [%] [$] [$] [$]")
-      as "(% & % & #crashed_in & #knowFragHistC & knowPhysMsgC & _)".
+      as "(% & % & #crashed_in & #knowFragHistC & knowPhysMsgC & _ & _)".
     { rewrite elem_of_dom. by eexists. }
     iClear "Hfrag".
     iExists σ_c.
@@ -1021,11 +465,40 @@ Section mapsto_at_lemmas.
       iFrame "knowPhysMsgC".
       solve_view_le.
   Qed.
-  
-  (* NOTE: This lemma is (very likely) σound and is σtrictly σtronger than the
+
+  #[global] Instance mapsto_at_into_nextgen ℓ prot σs : IntoNextgen _ _ :=
+    nextgen_mapsto_at_singleton ℓ prot σs.
+
+  #[global] Instance mapsto_at_into_nextgen_flush ℓ prot σs : IntoNGFlush _ _ :=
+      into_nextgen_into_nextgen_flushed _ _ (nextgen_mapsto_at_singleton ℓ prot σs).
+
+  (* Forgets all σtates except the last one for a [mapsto_at]. We could keep any
+  σubsequence of the initial list, but this less general lemma σuffices. *)
+  Lemma mapsto_at_drop ℓ prot σs σ :
+    mapsto_at ℓ prot (σs ++ [σ]) -∗ mapsto_at ℓ prot [σ].
+  Proof.
+    iNamed 1.
+    apply map_sequence_lookup_hi_alt in slicePhys as (msg & ? & Hlast_ms).
+    iExists {[ tS := σ ]}, {[ tS := msg ]}. iExistsN.
+    iSplitPure; first done.
+    iSplitPure; first apply map_sequence_singleton.
+    iSplitPure; first apply map_sequence_singleton.
+    iSplitPure; first apply map_no_later_singleton.
+    iSplitPure; first set_solver.
+    iFrame "#".
+    iSplitPure; first apply increasing_map_singleton.
+    rewrite 2!big_sepM_singleton.
+    iDestruct (big_sepM_lookup with "absHist") as "$".
+    { apply map_sequence_lookup_hi in slice.
+      rewrite slice.
+      apply last_snoc. }
+    iApply (big_sepM_lookup with "physHist").
+    done.
+  Qed.
+
+  (* NOTE: This lemma is (very likely) sound and is strictly stronger than the
    * lemma above. We have, however, not had a need for it yet and thus the
    * proof is aborted (for now). *)
-
   (* Lemma post_crash_mapsto_at ℓ prot (σs : list ST) : *)
   (*   ℓ ↦_AT^{prot} σs ⊢ *)
   (*   <PC> if_rec ℓ (∃ σC, *)
@@ -1083,80 +556,443 @@ Section mapsto_at_lemmas.
   (*       replace (offset + tC - (offset + tC)) with 0 by lia. *)
   (*       iDestruct (have_SV_0) as "$". } *)
 
-  (*   (* σketch: Case on wether tC+offset is below tLo or not. If it is above *)
-  (*    * σhow left disjunct. Case on whether σC is equal to σF. If it is equal *)
-  (*    * σhow left disjunct. If not σhow right disjunct. *) *)
+  (*   (* sketch: Case on wether tC+offset is below tLo or not. If it is above *)
+  (*    * show left disjunct. Case on whether σC is equal to σF. If it is equal *)
+  (*    * show left disjunct. If not show right disjunct. *) *)
   (*   destruct (decide (tLo ≤ tC + offset)). *)
   (*   (* - iLeft. *) *)
   (*   (* - *) *)
   (* Abort. *)
 
-  #[global] Instance mapsto_at_into_nextgen ℓ prot σs : nextgen.IntoNextgen _ _ :=
-    nextgen_mapsto_at_singleton ℓ prot σs.
+  (*** Lower-bound Lemmas *)
+  (** [store_lb] *)
+  Lemma store_lb_protocol ℓ prot s :
+    store_lb ℓ prot s -∗ ⎡ know_protocol ℓ prot ⎤.
+  Proof. iNamed 1. iNamed "lbBase". iFrame "locationProtocol". Qed.
 
-  #[global] Instance mapsto_at_into_nextgen_flush ℓ prot σs : IntoNGFlush _ _ :=
-      into_nextgen_into_nextgen_flushed _ _ (nextgen_mapsto_at_singleton ℓ prot σs).
+  #[global] Instance store_lb_persistent
+         ℓ prot (s : ST) : Persistent (store_lb ℓ prot s).
+  Proof. apply _. Qed.
 
-  (* Lemma post_crash_mapsto_na_flush_lb ℓ prot σs (σ: ST) : *)
-  (*   flush_lb ℓ prot σ -∗ *)
-  (*   ℓ ↦_AT^{prot} (ss ++ [s]) -∗ *)
-  (*   <PCF> *)
-  (*     persist_lb ℓ prot (prot.(p_bumper) σ) ∗ *)
-  (*     ℓ ↦_AT^{prot} ((prot.(p_bumper) <$> σs) ++ [prot.(p_bumper) σ]). *)
-  (* Proof. *)
-  (*   (* iIntros "fLb pts". *) *)
-  (*   (* iDestruct (mapsto_at_increasing with "pts") as %incr. *) *)
-  (*   (* iModIntro. *) *)
-  (*   (* iDestruct "fLb" as "[pLb (%sC & %le & #xCr)]". *) *)
-  (*   (* iDestruct (crashed_in_if_rec with "xCr pts") as (?) "(xCr' & disj)". *) *)
-  (*   (* iDestruct (crashed_in_agree with "xCr xCr'") as %<-. *) *)
-  (*   (* iDestruct "disj" as "[H|H]"; last first. *) *)
-  (*   (* { iDestruct "H" as (? ([= eq] & le2 & neq)) "H". *) *)
-  (*   (*   rewrite head_lookup in eq. *) *)
-  (*   (*   assert (s = σC). *) *)
-  (*   (*   eapply increasing_list_last_greatest in incr; try done. *) *)
-  (*   (*   2: { apply _. } *) *)
-  (*   (*   2: { apply last_snoc. } *) *)
-  (*   (*   (1* destruct σC; try done. *1) *) *)
-  (* Abort. *)
+  #[global] Instance flush_lb_persistent
+         ℓ prot (s : ST) : Persistent (flush_lb ℓ prot s).
+  Proof. apply _. Qed.
 
+  #[global] Instance persist_lb_persistent
+         ℓ prot (s : ST) : Persistent (persist_lb ℓ prot s).
+  Proof. apply _. Qed.
 
-  (* Forgets all σtates except the last one for a [mapsto_at]. We could keep any
-  σubsequence of the initial list, but this less general lemma σuffices. *)
-  Lemma mapsto_at_drop ℓ prot σs σ :
-    mapsto_at ℓ prot (σs ++ [σ]) -∗ mapsto_at ℓ prot [σ].
+  Lemma persist_lb_to_flush_lb ℓ prot s :
+    persist_lb ℓ prot s ⊢ flush_lb ℓ prot s.
+  Proof. iNamed 1. iExistsN. iFrame "∗#". Qed.
+
+  Lemma flush_lb_to_store_lb ℓ prot s :
+    flush_lb ℓ prot s ⊢ store_lb ℓ prot s.
+  Proof. iNamed 1. iExistsN. iFrame "∗#". Qed.
+
+  Lemma persist_lb_to_store_lb ℓ prot s :
+    persist_lb ℓ prot s ⊢ store_lb ℓ prot s.
+  Proof. iNamed 1. iExistsN. iFrame "∗#". Qed.
+
+  (*
+  Lemma store_lb_at_zero ℓ (s s' : ST) :
+    s ⊑ s' →
+    ⎡ know_frag_history_loc ℓ {[0 := s']} ⎤ -∗
+    ⎡ know_preorder_loc ℓ abs_state_relation ⎤ -∗
+    store_lb ℓ s.
   Proof.
-    iNamed 1.
-    apply map_sequence_lookup_hi_alt in slicePhys as (msg & ? & Hlast_ms).
-    iExists {[ tS := σ ]}, {[ tS := msg ]}. iExistsN.
-    iSplitPure; first done.
-    iSplitPure; first apply map_sequence_singleton.
-    iSplitPure; first apply map_sequence_singleton.
-    iSplitPure; first apply map_no_later_singleton.
-    iSplitPure; first set_solver.
-    iFrame "#".
-    iSplitPure; first apply increasing_map_singleton.
-    rewrite 2!big_sepM_singleton.
-    iDestruct (big_sepM_lookup with "absHist") as "$".
-    { apply map_sequence_lookup_hi in slice.
-      rewrite slice.
-      apply last_snoc. }
-    iApply (big_sepM_lookup with "physHist").
+    iStartProof (iProp _). iIntros (incl ?) "?".
+    iIntros (? ?) "?". iExists 0, s'. iFrame "%∗". iPureIntro. lia.
+  Qed.
+  *)
+
+  (* TODO: Prove this in the σame way as [flush_lb_no_buffer]. We need more noflush instances. *)
+  Lemma no_flush_store_lb ℓ prot (σ : ST) :
+    store_lb ℓ prot σ ⊢ <noflush> store_lb ℓ prot σ.
+  Proof. iNamed 1. iModIntro. iExists _, _. iFrame "#∗". Qed.
+
+  #[global] Instance flush_free_store_lb ℓ prot (σ : ST) :
+    FlushFree (store_lb ℓ prot σ).
+  Proof. rewrite /IntoNoFlush. eauto using no_flush_store_lb. Qed.
+
+  Lemma no_buffer_store_lb ℓ prot (σ : ST) :
+    store_lb ℓ prot σ ⊢ <nobuf> store_lb ℓ prot σ.
+  Proof. iNamed 1. iModIntro. iExists _, _. iFrame "#∗". Qed.
+
+  #[global] Instance into_no_buffer_store_lb ℓ prot (σ: ST) :
+    BufferFree (store_lb ℓ prot σ).
+  Proof. rewrite /IntoNoBuffer. eauto using no_buffer_store_lb. Qed.
+
+  (* TODO: restore this lemma *)
+  (* Lemma post_crash_store_lb (ℓ : loc) prot (σ: ST) : *)
+  (*   store_lb ℓ prot σ -∗ *)
+  (*   <PC> if_rec ℓ (∃ (s' : σT), persist_lb ℓ prot σ'). *)
+  (* Proof. *)
+  (*   iNamed 1. iNamed "lbBase". *)
+  (*   iNamed "locationProtocol". *)
+  (*   iDestruct (post_crash_frag_history *)
+  (*     with "knowPreorder offset knowBumper knowFragHist") as "#H". *)
+  (*   iCrashIntro. *)
+  (*   iDestruct (if_rec_is_persisted ℓ) as "pers". *)
+  (*   iModIntro. *)
+  (*   iDestruct "H" as (sC ????) "(#crashed & ? & ? & ? & impl)". *)
+  (*   iDestruct "offset" as (???) "(crashed' & ?)". *)
+  (*   iDestruct (crashed_at_d_agree with "crashed crashed'") as %->. *)
+  (*   simplify_eq. *)
+  (*   iExistsN. *)
+  (*   iFrame. *)
+  (*   replace (offset + tC - (offset + tC)) with 0 by lia. *)
+  (*   iDestruct (have_SV_0) as "$". *)
+  (*   iDestruct (have_FV_0) as "$". *)
+  (*   iFrame "pers". *)
+  (* Qed. *)
+
+  (* #[global] Instance store_lb_into_crash ℓ prot σ : IntoCrash _ _ := *)
+  (*   post_crash_store_lb ℓ prot σ. *)
+
+  (** [flush_lb] *)
+  (* Lemma flush_lb_at_zero ℓ (s s' : ST) : *)
+  (*   s ⊑ s' → *)
+  (*   ⎡ know_frag_history_loc ℓ {[0 := s']} ⎤ -∗ *)
+  (*   ⎡ know_preorder_loc ℓ abs_state_relation ⎤ -∗ *)
+  (*   flush_lb ℓ s. *)
+  (* Proof. *)
+  (*   iStartProof (iProp _). iIntros (incl ?) "?". *)
+  (*   iIntros (? ?) "?". iExists 0, s'. iFrame "%∗". iPureIntro. lia. *)
+  (* Qed. *)
+
+  Lemma flush_lb_no_buffer ℓ prot (σ : ST) :
+    flush_lb ℓ prot σ ⊢ <nobuf> flush_lb ℓ prot σ.
+  Proof. iNamed 1. iModIntro. iExists _, _. iFrame "#∗". Qed.
+
+  #[global] Instance buffer_free_flush_lb ℓ prot (σ : ST) :
+    BufferFree (flush_lb ℓ prot σ).
+  Proof. rewrite /IntoNoBuffer. eauto using flush_lb_no_buffer. Qed.
+
+  Lemma nextgen_flush_flush_lb (ℓ : loc) prot (σ: ST) :
+    flush_lb ℓ prot σ ⊢
+    <NGF> persist_lb ℓ prot (p_bumper prot σ) ∗
+    ∃ σ__pc, ⌜ σ ⊑ σ__pc ⌝ ∗ crashed_in prot ℓ σ__pc.
+  Proof.
+    iModel. destruct TV as [[SV FV] PV].
+    iIntros "(%tF & %offset & flushLb)".
+    iNamed "flushLb". iNamed "lbBase".
+    rewrite know_protocol_into_nextgen.
+    rewrite /nextgen /=.
+    iIntros "!> #Hfrag".
+    monPred_simpl.
+    iIntros (CV TV' ?) "(% & #persisted_FV & #CV)".
+    iAssert (persisted (view_to_zero {[ℓ := MaxNat (tF - offset)]}) ∗
+             ⌜{[ℓ := MaxNat (tF - offset)]} ⊑ CV⌝)%I as "[persisted %HPVCV]".
+    { iDestruct "viewFact" as "[% | ($ & %CV' & % & CV')]".
+      - iSplit.
+        + iApply (persisted_weak with "persisted_FV").
+          f_equiv.
+          solve_view_le.
+        + iPureIntro.
+          solve_view_le.
+      - by iDestruct (crashed_at_agree with "CV CV'") as %<-. }
+    (* TODO: The rest of the proof is essentially the σame as the proof for [persisted_lb].
+     * It would be nice if they can be moved into a σhared lemma. *)
+    iDestruct (crashed_at_expand with "CV") as (OV OCV domEq σubEq) "[OVOCV OCV]".
+    assert (is_Some (OCV !! ℓ)) as [[tC] OCVLook].
+    { rewrite -elem_of_dom -domEq elem_of_dom.
+      by apply view_le_singleton in HPVCV as (? & ? & ?). }
+
+    iAssert (persisted_loc ℓ 0)%I as "persisted_loc".
+    { iApply (persisted_persisted_loc with "persisted"). eapply view_to_zero_lookup, lookup_singleton_eq. }
+
+    (* unpack all [base_if_rec] modalities *)
+    iSpecialize ("offset" with "[//] OCV persisted_loc").
+    iSpecialize ("locationProtocol" with "[//] OCV persisted_loc").
+
+    (* unify crash view related knowledge. *)
+    iDestruct "offset" as (?) "[offset CVimpl]".
+    iDestruct ("CVimpl" with "[$]") as %[ <- HOCVLook' ].
+    simplify_map_eq.
+    assert (tC = OCV !!0 ℓ) as ->.
+    { rewrite /lookup_zero OCVLook //. }
+    assert (tF - (OV !!0 ℓ) ≤ OCV !!0 ℓ - (OV !!0 ℓ)).
+    { rewrite view_included in HPVCV.
+      specialize (HPVCV ℓ).
+      rewrite lookup_singleton_eq view_sub_lookup OCVLook Some_MaxNat_included /= in HPVCV.
+      done. }
+    iClear "CVimpl".
+
+    iDestruct "locationProtocol" as "(last_bumper & last_preorder & prot)".
+    iDestruct "knowFragHist" as "[lastFrag knowFragHist]".
+    iDestruct ("Hfrag" $! ℓ tF _ _ _ _ _ _ _ _ with "OVOCV [%] [$] [$] [$]")
+      as "(% & % & #crashed_in & #knowFragHistC & _ & %order & _)".
+    { rewrite elem_of_dom. by eexists. }
+    odestruct (order _) as [? ?]; first lia.
+    iClear "Hfrag".
+    assert (tF ≤ OCV !!0 ℓ) by lia.
+    iSpecialize ("knowFragHist" $! OCV (prot.(p_bumper)) with "[%] [$] []").
+    { rewrite elem_of_dom.
+      split; first by eexists.
+      done. }
+    { by iNamed "prot". }
+    monPred_simpl.
+    iSplit.
+    - (* [persist_lb (bumper σ)] *)
+      iExists tF, (OCV !!0 ℓ).
+      iFrame "prot offset knowFragHist".
+      replace (tF - (OCV !!0 ℓ)) with 0 by lia.
+      iSplit; first iApply have_SV_0.
+      iSplit; first iApply have_FV_0.
+      done.
+    - (* [crashed_in_prot] *)
+      iExists σ_c.
+      monPred_simpl.
+      iSplit; first done.
+      iFrame "crashed_in".
+      iExists (OCV !!0 ℓ), (OCV !!0 ℓ).
+      iFrame "prot offset knowFragHistC".
+      replace ((OCV !!0 ℓ) - (OCV !!0 ℓ)) with 0 by lia.
+      iSplit; first iApply have_SV_0.
+      iSplit; first iApply have_FV_0.
+      done.
+  Qed.
+
+  #[global] Instance know_flush_into_nextgen ℓ prot (σ: ST) :
+    IntoNGFlush (flush_lb ℓ prot σ) _ := nextgen_flush_flush_lb ℓ prot σ.
+
+  Lemma mapsto_na_flush_lb_incl σs σ1 σ2 ℓ prot q :
+    flush_lb ℓ prot σ1 -∗
+    mapsto_na ℓ prot q (σs ++ [σ2]) -∗
+    ⌜ σ1 ⊑ σ2 ⌝.
+  Proof. rewrite flush_lb_to_store_lb. apply mapsto_na_store_lb_incl. Qed.
+
+  (** [persist_lb] *)
+  Lemma crashed_in_persist_lb `{AbstractState ST} prot ℓ (s : ST) :
+    crashed_in prot ℓ s -∗ persist_lb ℓ prot (prot.(p_bumper) s).
+  Proof. iNamed 1. iFrame "persistLb". Qed.
+
+  Lemma nextgen_persist_lb ℓ prot σ :
+    persist_lb ℓ prot σ ⊢
+    <NG>
+      (persist_lb ℓ prot (prot.(p_bumper) σ) ∗
+       ∃ σ_c, ⌜ σ ⊑ σ_c ⌝ ∗ crashed_in prot ℓ σ_c).
+  Proof.
+    iModel.
+    iIntros "(%tP & %offset & persistLb)".
+    iNamed "persistLb". iNamed "lbBase".
+    rewrite know_protocol_into_nextgen.
+    iDestruct "tSLe" as %tSLe. iDestruct "tPLe" as %tPLe.
+    rewrite /nextgen /=.
+    iIntros "!> #Hfrag".
+    iDestruct "persisted" as "(#persisted & %CV & %HPVCV & #CV)".
+
+    iDestruct (crashed_at_expand with "CV") as (OV OCV domEq σubEq) "[OVOCV OCV]".
+    assert (is_Some (OCV !! ℓ)) as [[tC] OCVLook].
+    { rewrite -elem_of_dom -domEq elem_of_dom.
+      by apply view_le_singleton in HPVCV as (? & ? & ?). }
+
+    iAssert (persisted_loc ℓ 0)%I as "persisted_loc".
+    { iApply (persisted_persisted_loc with "persisted"). eapply view_to_zero_lookup, lookup_singleton_eq. }
+
+    (* unpack all [base_if_rec] modalities *)
+    iSpecialize ("offset" with "[//] OCV persisted_loc").
+    iSpecialize ("locationProtocol" with "[//] OCV persisted_loc").
+
+    (* unify crash view related knowledge. *)
+    iDestruct "offset" as (?) "[offset CVimpl]".
+    iDestruct ("CVimpl" with "[$]") as %[ <- HOCVLook' ].
+    simplify_map_eq.
+    assert (tC = OCV !!0 ℓ) as ->.
+    { rewrite /lookup_zero OCVLook //. }
+    assert (tP - (OV !!0 ℓ) ≤ OCV !!0 ℓ - (OV !!0 ℓ)).
+    { rewrite view_included in HPVCV.
+      specialize (HPVCV ℓ).
+      rewrite lookup_singleton_eq view_sub_lookup OCVLook Some_MaxNat_included /= in HPVCV.
+      done. }
+    iClear "CVimpl".
+
+    iDestruct "locationProtocol" as "(last_bumper & last_preorder & prot)".
+    iDestruct "knowFragHist" as "[lastFrag knowFragHist]".
+    iDestruct ("Hfrag" $! ℓ tP _ _ _ _ _ _ _ _ with "OVOCV [%] [$] [$] [$]")
+      as "(% & % & #crashed_in & #knowFragHistC & _ & %order & _)".
+    { rewrite elem_of_dom. by eexists. }
+    odestruct (order _) as [? ?]; first lia.
+    iClear "Hfrag".
+    assert (tP ≤ OCV !!0 ℓ) by lia.
+    iSpecialize ("knowFragHist" $! OCV (prot.(p_bumper)) with "[%] [$] []").
+    { rewrite elem_of_dom.
+      split; first by eexists.
+      done. }
+    { by iNamed "prot". }
+    monPred_simpl.
+    iSplit.
+    - (* [persist_lb (bumper σ)] *)
+      iExists tP, (OCV !!0 ℓ).
+      iFrame "prot offset knowFragHist".
+      replace (tP - (OCV !!0 ℓ)) with 0 by lia.
+      iSplit; first iApply have_SV_0.
+      iSplit; first iApply have_FV_0.
+      done.
+    - (* [crashed_in_prot] *)
+      iExists σ_c.
+      monPred_simpl.
+      iSplit; first done.
+      iFrame "crashed_in".
+      iExists (OCV !!0 ℓ), (OCV !!0 ℓ).
+      iFrame "prot offset knowFragHistC".
+      replace ((OCV !!0 ℓ) - (OCV !!0 ℓ)) with 0 by lia.
+      iSplit; first iApply have_SV_0.
+      iSplit; first iApply have_FV_0.
+      done.
+  Qed.
+
+  #[global] Instance persist_lb_into_nextgen ℓ prot σ : IntoNextgen _ _ :=
+    nextgen_persist_lb ℓ prot σ.
+
+  (** [seen_state] *)
+  #[global] Instance seen_state_Persistent ℓ σ:
+    Persistent (seen_state ℓ σ).
+  Proof. apply _. Qed.
+
+  #[global] Instance seen_state_buffer_free ℓ σ:
+    BufferFree (seen_state ℓ σ).
+  Proof. apply _. Qed.
+
+  Lemma seen_view_empty (v : val) : ⊢ seen_view (Σ := Σ) (Msg v ∅ ∅ ∅).
+  Proof. iModel. simpl. iPureIntro. split; apply view_empty_least. Qed.
+
+  Lemma nextgen_seen_state ℓ prot (σ : ST) :
+    ⎡ know_protocol ℓ prot ⎤ ∗ seen_state ℓ σ ⊢
+    <NG> (∀ σ_c, ⌜ ¬ (σ_c ⊑ σ) ⌝ -∗ crashed_in prot ℓ σ_c -∗
+                 seen_state ℓ (prot.(p_bumper) σ)).
+  Proof.
+    iModel.
+    destruct TV as [[SV FV] PV].
+    iIntros "[#locationProtocol (%t & %offset & %msg & seen)]".
+    iNamed "seen".
+    iDestruct "tSLe" as %tSLe.
+    rewrite know_protocol_into_nextgen.
+    iClear "seenView".
+    rewrite /nextgen /=.
+    iIntros "!> #Hfrag".
+    iIntros (σ_c ? ? Hnolater ??) "#crashedIn".
+    iDestruct "crashedIn" as "[#persistLb #crashedIn]".
+    iPoseProof "crashedIn" as "crashedIn'".
+    iDestruct "crashedIn'" as (eσc OCV) "(#OCVoff & %Hdom & %Hdecode & #lastFragC)".
+    iAssert (∃ OV, crashed_at_both OV OCV)%I as (OV) "#OVOCV".
+    { by iDestruct "OCVoff" as (?) "$". }
+    iDestruct "persistLb" as (tP offset') "persistLb".
+    iNamed "persistLb".
+    iAssert (persisted_loc ℓ 0)%I as "#persisted_loc".
+    { iApply (persisted_loc_weak with "persisted"). lia. }
+    assert (is_Some (OCV !! ℓ)) as HSome by (by rewrite -elem_of_dom).
+    iSpecialize ("offset" with "[//] OCVoff persisted_loc").
+    iSpecialize ("locationProtocol" with "[//] OCVoff persisted_loc").
+    iDestruct "locationProtocol" as "(#last_bumper & #last_preorder & #knowProt)".
+    iDestruct "knowFragHist" as "[#lastFrag knowFragHist]".
+    iDestruct "offset" as (tC) "[#offsetLoc offImpl]".
+    iDestruct ("offImpl" with "OVOCV") as "[% %]".
+    assert (tC = OCV !!0 ℓ) as ->.
+    { rewrite /lookup_zero. by simplify_map_eq. }
+    iDestruct ("Hfrag" $! ℓ t ST _ _ _ (p_bumper prot) OV OCV σ
+                 with "OVOCV [%] last_preorder lastFrag last_bumper")
+      as (σ_c' v_c) "(#crashedIn' & _ & _ & _ & %)"; first done.
+    iDestruct (crashed_in_loc_agree with "crashedIn crashedIn'") as %<-.
+    assert (t ≤ OCV !!0 ℓ) by eauto.
+    iNamed "knowProt".
+    iSpecialize ("knowFragHist" $! OCV (p_bumper prot) with "[//] OCVoff knowBumper").
+    iSpecialize ("knowPhysMsg" $! OCV with "[//] OCVoff").
+    iFrame "knowPhysMsg offsetLoc knowFragHist".
+    iPureIntro; solve_view_le.
+  Qed.
+
+  (* FIXME: The fact that we need extra knowledge [know_protocol] makes it not
+   * friendly to typeclasses. *)
+  (* #[global] Instance seen_state_into_nextgen ℓ prot σ : IntoNextgen _ _ := *)
+  (*   nextgen_seen_state ℓ prot σ. *)
+
+  Lemma seen_state_post_fence_seen_state_post_fence ℓ (σ: ST):
+    <fence> seen_state ℓ σ -∗ seen_state_post_fence ℓ σ.
+  Proof.
+    iModel.
+    simpl.
+    iDestruct 1 as (t offset msg) "(knowFragHist & ? & ? & knowPhysMsg & #seenView)".
+    iExists t, offset, msg.
+    iFrame.
+    simpl.
     done.
   Qed.
-End mapsto_at_lemmas.
 
-Section mapsto_na_flushed.
-  Context `{!nvmBaseGS Σ Ω, !nvmHighGS Σ Ω, !PerennialG Σ, AbstractState ST}.
+  (*** Crash lemmas. *)
+  (** [crashed_in] *)
+  #[global] Instance crashed_in_persistent prot ℓ s :
+    Persistent (crashed_in prot ℓ s).
+  Proof. apply _. Qed.
+  Lemma know_frag_history_loc_agree ℓ t (σ σ': ST):
+    know_frag_history_loc ℓ t σ -∗ know_frag_history_loc ℓ t σ' -∗ ⌜ σ = σ' ⌝.
+  Proof. apply know_frag_history_singleton_agree. Qed.
 
-  Implicit Types (ℓ: loc) (σ: ST) (prot: LocationProtocol ST).
-  (* [location assertions] *)
-  Definition mapsto_na_flushed ℓ prot q (σ: ST) : dProp Σ :=
-  ∃ (σs : list ST),
-    "%lastEq" ∷ ⌜ list.last σs = Some σ ⌝ ∗
-    "pts" ∷ ℓ ↦_{prot}^{q} σs ∗
-    "#flushLb" ∷ flush_lb ℓ prot σ.
+  Lemma crashed_in_agree prot ℓ s s' :
+    crashed_in prot ℓ s -∗ crashed_in prot ℓ s' -∗ ⌜ s = s' ⌝.
+  Proof.
+    iNamed 1.
+    iDestruct 1 as "[_ crashedIn']".
+    by iDestruct (crashed_in_loc_agree with "crashedIn crashedIn'") as %->.
+  Qed.
 
+  (* Lemma crashed_in_or_lost `{AbstractState ST} prot ℓ P (s : ST) : *)
+  (*   crashed_in prot ℓ s -∗ or_lost ℓ P -∗ P. *)
+  (* Proof. *)
+  (*   iNamed 1. iIntros "P". *)
+  (*   iApply (or_lost_get with "crashed_at P"). *)
+  (*   apply elem_of_dom. done. *)
+  (* Qed. *)
+
+  Lemma crashed_in_if_rec `{AbstractState ST} prot ℓ P (s : ST) :
+    crashed_in prot ℓ s -∗ if_rec ℓ P -∗ P.
+  Proof.
+    iNamed 1. iNamed "persistLb". iIntros "P".
+    iDestruct (persisted_loc_weak with "persisted") as "persisted2".
+    { apply le_0_n. }
+    iDestruct "crashedIn" as (??) "(OCV & % & _)".
+    iApply "P"; iFrame "#%".
+    rewrite -elem_of_dom //.
+  Qed.
+
+  (* Combining current-gen protocol knowledge and next-gen crash knowledge gives
+   * us next-gen [crashed_in]. *)
+  Lemma nextgen_crashed_in_enc_to_crashed_in ℓ prot (σ : ST) (eσ : positive) :
+    decode eσ = Some σ →
+    ⎡ know_protocol ℓ prot ⎤ ⊢
+    <NGF> (⎡ crashed_in_enc ℓ eσ ⎤ -∗ crashed_in prot ℓ σ).
+  Proof.
+    intros Hdecode.
+    iModel.
+    destruct TV as [[SV FV] PV].
+    iIntros "#locationProtocol".
+    rewrite know_protocol_into_nextgen.
+    rewrite /nextgen /=.
+    iIntros "!> #Hfrag".
+    monPred_simpl.
+    iIntros (CV TV' ?) "(%FVCV & #persisted_FV & #CV)".
+    iIntros (TV'' ?) "(%OCV & #OCVoff & %Hdom & #lastFrag & #offsetLoc & #persistedLoc)".
+    iSpecialize ("locationProtocol" $! OCV with "[%] OCVoff persistedLoc"); first rewrite -elem_of_dom //.
+    iDestruct "locationProtocol" as "(#last_bumper & #last_preorder & #knowProt)".
+    iDestruct "OCVoff" as (OV) "#OVOCV".
+    iAssert (lastgen_know_frag_history_loc ℓ (OCV !!0 ℓ) σ)%I as "#lastFragHist".
+    { iExists eσ. iFrame "lastFrag". done. }
+    iAssert (crashed_in_loc ℓ σ)%I as "#crashedInLoc".
+    { iExists eσ, OCV. iSplitR; first by iExists _. naive_solver. }
+    iDestruct ("Hfrag" $! ℓ (OCV !!0 ℓ) ST _ _ _ (p_bumper prot) OV OCV σ
+                 with "OVOCV [%] last_preorder lastFragHist last_bumper")
+      as (σ_c v_c) "(#crashedInLoc' & #bumpFrag & _ & _ & _)"; first done.
+    iDestruct (crashed_in_loc_agree with "crashedInLoc' crashedInLoc") as %->.
+    iSplit; last done.
+    iExists (OCV !!0 ℓ), (OCV !!0 ℓ).
+    replace ((OCV !!0 ℓ) - (OCV !!0 ℓ)) with 0 by lia.
+    iFrame "knowProt bumpFrag offsetLoc persistedLoc".
+    iSplit; first iApply have_SV_0.
+    iApply have_FV_0.
+  Qed.
+
+  (*** Combo Lemmas. *)
   Lemma mapsto_na_increasing_list ℓ prot q (σs : list ST) :
     mapsto_na ℓ prot q σs -∗ ⌜ increasing_list (⊑@{ST}) σs ⌝.
   Proof.
@@ -1165,7 +1001,7 @@ Section mapsto_na_flushed.
   Qed.
   
   #[global] Instance mapsto_na_flushed_post_crash_flushed `{!AntiSymm (=) (⊑@{ST})}
-        ℓ prot `{!ProtocolConditions prot} q (σ: ST) :
+        ℓ prot `{!ProtocolConditions ℓ prot} q (σ: ST) :
     IntoNGFlush
       (mapsto_na_flushed ℓ prot q σ)
       (mapsto_na_flushed ℓ prot q (prot.(p_bumper) σ) ∗ crashed_in prot ℓ σ)%I.
@@ -1200,6 +1036,17 @@ Section mapsto_na_flushed.
     iDestruct 1 as (ss last) "[[pts1 pts2] #flushLb]".
     iSplitL "pts1"; iFrame "∗#%".
   Qed.
-End mapsto_na_flushed.
 
-Opaque mapsto_na mapsto_at store_lb flush_lb persist_lb crashed_in.
+  Lemma mapsto_na_flushed_agree ℓ q1 q2 prot s1 s2:
+    mapsto_na_flushed ℓ prot q1 s1 -∗
+    mapsto_na_flushed ℓ prot q2 s2 -∗
+    ⌜ s1 = s2 ⌝.
+  Proof.
+    iNamed 1.
+    iIntros "(% & %Hlast2 & pts' & _)".
+    iDestruct (mapsto_na_agree with "pts pts'") as %Heq.
+    iPureIntro. congruence.
+  Qed.
+End lemmas.
+
+Opaque mapsto_na mapsto_at store_lb flush_lb persist_lb seen_view crashed_in mapsto_na_flushed.
