src/high/protocol.v
@@ -6,39 +6,14 @@ From self Require Import encode_relation.
 
 From self.high Require Import dprop generational_resources modalities monpred_simpl predicates.
 From self.high.resources Require Import gen_ghost_map.
-
+From self.high Require Export protocol_defs.
+From self.high Require Import locations_defs.
 From self.lang Require Import lang.
 
-(* A handy alias for the type of location predicates. *)
-Definition loc_pred `{nvmHighGS} ST `{AbstractState ST} := ST → val → dProp Σ.
-
-Definition loc_predO `{nvmHighGS} ST := ST -d> val -d> dPropO Σ.
-
-(* A protocol consists of
-  - A predicate [p_inv] that holds for each write and corresponding state of the
-    location.
-  - A function [bumper] that specifies how the state of a location changes
-    after a crash. *)
-
-Record LocationProtocol ST `{AbstractState ST, nvmHighGS} := MkProt {
-  p_full : loc_pred ST;
-  p_read : loc_pred ST;
-  p_pers : loc_pred ST;
-  p_bumper : ST → ST;
-}.
-
-#[global] Arguments MkProt   {ST _ _ _ _ _ _ _} _%_I _%_I _%_I _.
-#[global] Arguments p_full   {ST _ _ _ _ _ _ _} _.
-#[global] Arguments p_read   {ST _ _ _ _ _ _ _} _.
-#[global] Arguments p_pers   {ST _ _ _ _ _ _ _} _.
-#[global] Arguments p_bumper {ST _ _ _ _ _ _ _} _ _.
-
 (* Type class collection the properties that a protocol should have.
-
-Note: The fields are ordered by "difficulty" in the sense of how difficult these
-conditions usually are to show.  *)
-
-Class ProtocolConditions `{AbstractState ST, nvmHighGS} (prot : LocationProtocol ST) := {
+ * Note: The fields are ordered by "difficulty" in the sense of how difficult
+ * these conditions usually are to show. *)
+Class ProtocolConditions `{AbstractState ST, nvmHighGS} (ℓ : loc) (prot : LocationProtocol ST) := {
   bumper_mono :
     Proper ((⊑@{ST}) ==> (⊑))%signature (prot.(p_bumper));
   full_nobuf ::
@@ -50,99 +25,47 @@ Class ProtocolConditions `{AbstractState ST, nvmHighGS} (prot : LocationProtocol
   full_read_split :
     forall s v, prot.(p_full) s v ⊣⊢ prot.(p_read) s v ∗ (prot.(p_read) s v -∗ prot.(p_full) s v);
   pred_full_nextgen :
-    ⊢ ∀ σ_p v_p σ_f v_f, ⌜ σ_p ⊑ σ_f ⌝ -∗ prot.(p_pers) σ_p v_p -∗ prot.(p_full) σ_f v_f -∗
+    ⎡ know_protocol ℓ prot ⎤ ⊢
+      ∀ σ_p v_p σ_f v_f, ⌜ σ_p ⊑ σ_f ⌝ -∗ prot.(p_pers) σ_p v_p -∗ prot.(p_full) σ_f v_f -∗
       (* first case: we crash exactly at [σ_f] *)
-      (|==> <NGF> prot.(p_full) (prot.(p_bumper) σ_f) v_f ∗ prot.(p_pers) (prot.(p_bumper) σ_f) v_f) ∧
+      (|==> <NGF> crashed_in prot ℓ σ_f -∗
+            prot.(p_full) (prot.(p_bumper) σ_f) v_f ∗ prot.(p_pers) (prot.(p_bumper) σ_f) v_f) ∧
       (* second case: we crash later than [s_p] (included) but before [s] (excluded) *)
       (∀ σ_c v_c,
          (* We cannot take subjective resource from [p_full],
           * but we can take subjective resource from [p_read]. *)
          <obj> (prot.(p_read) σ_c v_c -∗ ⌜ σ_p ⊑ σ_c ⌝ -∗ ⌜ σ_c ⊑ σ_f ⌝ ==∗
-                <NGF> prot.(p_full) (prot.(p_bumper) σ_c) v_c ∗ prot.(p_pers) (prot.(p_bumper) σ_c) v_c));
+                <NGF> crashed_in prot ℓ σ_c -∗
+                      prot.(p_full) (prot.(p_bumper) σ_c) v_c ∗ prot.(p_pers) (prot.(p_bumper) σ_c) v_c));
   pred_read_nextgen :
     ⊢ ∀ s v, prot.(p_read) s v -∗ <NGF> prot.(p_read) (prot.(p_bumper) s) v
 }.
 
-#[global] Hint Mode ProtocolConditions + + + + + + + + ! : typeclass_instances.
+#[global] Hint Mode ProtocolConditions + + + + + + + + - ! : typeclass_instances.
 
 Existing Instance full_nobuf.
 Existing Instance read_nobuf.
 Existing Instance pers_obj.
 Existing Instance bumper_mono.
 
-(** [know_protocol] represents the knowledge that a location is associated with a
-specific protocol. It's defined simply using more "primitive" assertions. *)
-Definition know_protocol `{AbstractState ST, nvmHighGS}
-           ℓ (prot : LocationProtocol ST) : iProp Σ :=
-  "#knowFullPred" ∷  know_full_pred ℓ prot.(p_full)  ∗
-  "#knowReadPred" ∷  know_read_pred ℓ prot.(p_read)  ∗
-  "#knowPersPred" ∷  know_pers_pred ℓ prot.(p_pers)  ∗
-  "#knowPreorder" ∷  know_preorder_loc ℓ (⊑@{ST})  ∗
-  "#knowBumper" ∷  know_bumper ℓ prot.(p_bumper) .
+(* Helpers shared by the [na]/[at] allocation proofs (and used to discharge the
+   injected [crash_witness_enc] condition of [predFullNextgen]). *)
+Section encoding_lemmas.
+  Context `{AbstractState ST}.
+  Context `{nvmHighGS}.
 
-Lemma encode_bumper_bump_mono `{AbstractState ST}
-      (bumper : ST → ST) `{!Proper ((⊑@{ST}) ==> (⊑))%signature bumper}
-      (x y x' y' : positive) :
-  encode_bumper bumper x = Some x' →
-  encode_bumper bumper y = Some y' →
-  encode_relation (⊑@{ST}) x y →
-  encode_relation (⊑@{ST}) x' y'.
-Proof.
-  rewrite /encode_bumper. rewrite /encode_relation.
-  intros (sx & -> & <-)%encode_bumper_Some_decode.
-  intros (sy & -> & <-)%encode_bumper_Some_decode.
-  rewrite !decode_encode /=.
-  solve_proper.
-Qed.
+  Lemma know_protocol_enc_know_protocol ℓ (prot : LocationProtocol ST) :
+    Proper ((⊑@{ST}) ==> (⊑)) prot.(p_bumper) →
+    know_protocol_enc ℓ (encode_predicate prot.(p_full)) (encode_predicate prot.(p_read))
+      (encode_predicate prot.(p_pers)) (encode_relation (⊑@{ST}))
+      (encode_bumper prot.(p_bumper))
+    ⊢ know_protocol ℓ prot.
+  Proof. by iIntros "% ($ & $ & $ & $ & $)". Qed.
 
-Section protocol.
-  Context `{nvmHighGS, AbstractState ST}.
-
-  Implicit Types (prot : LocationProtocol ST).
-
-  #[local] Existing Instance nvmHighGS_inG.
-  #[local] Existing Instance nvmHighGpreS_bumpers.
-  
-  Lemma nextgen_know_protocol ℓ prot :
-    know_protocol ℓ prot -∗
-    ⚡==> base_if_rec ℓ (lastgen_know_bumper ℓ prot.(p_bumper) ∗ lastgen_know_preorder_loc ℓ (⊑@{ST}) ∗ know_protocol ℓ prot).
-  Proof.
-    iNamed 1.
-    iPoseProof (ghost_map_elem_into_nextgen_ifrec with "knowPreorder") as "knowPreorder'".
-    iPoseProof (ghost_map_elem_into_nextgen_ifrec with "[]") as "knowBumper'".
-    { iDestruct "knowBumper" as "[? $]". }
-    iDestruct "knowBumper" as "[% _]".
-    iModIntro.
-    iDestruct "knowBumper'" as "[$ knowBumper']".
-    iDestruct "knowPreorder'" as "[$ knowPreorder']".
-    rewrite -?if_rec_lift_if_rec.
-    
-    iModIntro. iFrame "#%".
-  Qed.
-
-  #[global] Instance know_protocol_into_nextgen ℓ prot :
-    base_IntoNextgen
-      ( know_protocol ℓ prot )
-      (base_if_rec ℓ (lastgen_know_bumper ℓ prot.(p_bumper) ∗ lastgen_know_preorder_loc ℓ (⊑@{ST}) ∗ know_protocol ℓ prot )).
-  Proof.
-    rewrite /base_IntoNextgen.
-    iIntros "P".
-    by iApply nextgen_know_protocol.
-  Qed.
-
-  #[global] Instance know_protocol_contractive ℓ bumper :
-    Contractive (λ (invs : (prodO (prodO (loc_predO ST) (loc_predO ST)) (loc_predO ST))),
-                      let '(full, read, pers) := invs in
-                      (know_protocol ℓ (MkProt full read pers bumper))).
-  Proof.
-    rewrite /know_protocol.
-    intros ????.
-    destruct x as [[full read] pers].
-    destruct y as [[full' read'] pers'].
-    simpl.
-    repeat
-      (done ||
-       f_contractive ||
-       f_equiv); apply H2.
-  Qed.
-End protocol.
+  Lemma know_protocol_know_protocol_enc ℓ (prot : LocationProtocol ST) :
+    know_protocol ℓ prot ⊢
+    know_protocol_enc ℓ (encode_predicate prot.(p_full)) (encode_predicate prot.(p_read))
+                        (encode_predicate prot.(p_pers)) (encode_relation (⊑@{ST}))
+                        (encode_bumper prot.(p_bumper)).
+  Proof. iIntros "($ & $ & $ & $ & [_ $])". Qed.
+End encoding_lemmas.
