src/high/locations_defs.v
@@ -1,0 +1,219 @@
+From iris_named_props Require Import named_props.
+From iris.proofmode Require Import proofmode.
+
+From self Require Import solve_view_le.
+From self.lang Require Import lang.
+From self.high Require Import generational_resources dprop protocol_defs.
+From self.high.modalities Require Import no_buffer no_flush.
+From self.high.lib Require Import abstract_state increasing_map.
+
+Section location_assertions.
+  Context `{nvmHighGS, AbstractState ST}.
+
+  Implicit Types (ℓ : loc) (σ : ST) (σs : list ST) (prot : LocationProtocol ST).
+  (*** mapsto predicates *)
+  (* Points-to predicate for non-atomics. This predcate says that we know that
+     the last events at [ℓ] corresponds to the last element in list [σs] *)
+  (* FIXME: Can [mapsto_na] use [lb_base]? *)
+  Definition mapsto_na (ℓ : loc) prot (q : frac) (σs : list ST) : dProp Σ :=
+    (∃ (tLo tHi offset : time) SV (abs_hist : gmap time ST) (msg : message) σ,
+      "%lastEq" ∷ ⌜ list.last σs = Some σ ⌝ ∗
+      "#locationProtocol" ∷ ⎡ know_protocol ℓ prot ⎤ ∗
+      "%incrMap" ∷ ⌜ increasing_map (⊑@{ST}) abs_hist ⌝ ∗
+      "#isNaLoc" ∷ ⎡ is_na_loc ℓ ⎤ ∗
+
+      (* [tHi] is the last message and it agrees with the last state in ss. *)
+      "%lookupV" ∷ ⌜ abs_hist !! tHi = Some σ ⌝ ∗
+      "%nolater" ∷ ⌜ map_no_later abs_hist tHi ⌝ ∗
+
+      (* Ownership over the full abstract history. *)
+      "hist" ∷ ⎡ know_full_history_loc ℓ q abs_hist ⎤ ∗
+      "#histFrag" ∷ ⎡ know_frag_history_loc ℓ tHi σ ⎤ ∗
+      (* "#offset" ∷ ⎡ ℓ ↪[offset_name]□ offset ⎤ ∗ *)
+      "#offset" ∷ ⎡ offset_loc ℓ offset ⎤ ∗
+
+      "knowSV" ∷ ⎡ know_na_view ℓ q SV ⎤ ∗
+      "%slice" ∷ ⌜ map_sequence abs_hist tLo tHi σs ⌝ ∗
+      "#physMsg" ∷ ⎡ know_phys_hist_msg ℓ tHi msg ⎤ ∗
+      "#inThreadView" ∷ have_thread_view (SV, msg_persisted_after_view msg, ∅) ∗
+      (* We have the [tHi] timestamp in our store view. *)
+      "%offsetLe" ∷ ⌜ offset ≤ tHi ⌝ ∗
+      "%haveTStore" ∷ ⌜ tHi - offset ≤ SV !!0 ℓ ⌝ ∗
+      "#pers" ∷ (⎡ persisted_loc ℓ (tLo - offset) ⎤ ∨ ⌜ tLo - offset = 0 ⌝)
+    )%I.
+
+  Program Definition have_msg_post_fence msg : dProp Σ :=
+    MonPred (λ TV,
+      ⌜ msg.(msg_store_view) ⊑ (store_view TV) ⌝
+      ∗
+      ⌜ msg.(msg_persisted_after_view) ⊑ (flush_view TV ⊔ buffer_view TV) ⌝
+    )%I _.
+  Next Obligation. solve_proper. Qed.
+
+  Program Definition have_msg_store_view msg : dProp Σ :=
+    MonPred (λ TV,
+      ⌜ msg.(msg_store_view) ⊑ (store_view TV) ⌝
+      (* ∗ *)
+      (* ⌜ msg.(msg_persisted_after_view) ⊑ (flush_view i.1 ⊔ buffer_view i.1) ⌝ *)
+    )%I _.
+  Next Obligation. solve_proper. Qed.
+
+  (** The following lemmas/instances cannot infer [Σ] when proved in a different context.
+   ** They are otherwise not used as definitions. *)
+  (* This is a revived [have_msg_after_fence] before the commit 96f65f5.
+   * We (maybe?) need this stronger version in order to extract resource
+   * from [p_read] into thread local view. *)
+  Lemma have_msg_post_fence_empty v PV : ⊢ have_msg_post_fence (Msg v ∅ PV ∅).
+  Proof.
+    iModel. simpl. iPureIntro. split; apply view_empty_least.
+  Qed.
+
+  (* and for the original assertion, I'm changing its name to be more explicit. *)
+  #[global] Instance have_msg_post_fence_persistent msg :
+    Persistent (have_msg_post_fence msg).
+  Proof. apply monPred_persistent=> j. apply _. Qed.
+
+  #[global] Instance have_msg_store_view_persistent msg :
+    Persistent (have_msg_store_view msg).
+  Proof. apply monPred_persistent=> j. apply _. Qed.
+
+  #[global] Instance have_msg_store_view_buffer_free msg :
+    BufferFree (have_msg_store_view msg).
+  Proof. rewrite /IntoNoBuffer. iModel. done. Qed.
+
+  #[global] Instance have_msg_store_view_flush_free msg :
+    FlushFree (have_msg_store_view msg).
+  Proof. rewrite /IntoNoFlush. iModel. done. Qed.
+
+  Lemma have_msg_store_view_empty v PV : ⊢ have_msg_store_view (Msg v ∅ PV ∅).
+  Proof.
+    iModel. simpl. iPureIntro. apply view_empty_least.
+  Qed.
+
+  Definition mapsto_at ℓ prot ss : dProp Σ :=
+    (∃ (abs_hist : gmap time ST) (phys_hist : gmap time message) tLo tS offset s ms,
+        "%lastEq" ∷ ⌜ list.last ss = Some s ⌝ ∗ (* NOTE: Could we change this to non-empty? *)
+        "%slice" ∷ ⌜ map_sequence abs_hist tLo tS ss ⌝ ∗
+        "%slicePhys" ∷ ⌜ map_sequence phys_hist tLo tS ms ⌝ ∗
+        "%nolater" ∷ ⌜ map_no_later abs_hist tS ⌝ ∗
+        "%absPhysHistDomEq" ∷ ⌜ dom abs_hist = dom phys_hist ⌝ ∗
+        "#isAtLoc" ∷ ⎡ is_at_loc ℓ ⎤ ∗
+        "#locationProtocol" ∷ ⎡ know_protocol ℓ prot ⎤ ∗
+        "%incrMap" ∷ ⌜ increasing_map (⊑@{ST}) abs_hist ⌝ ∗
+        "#absHist" ∷
+          ([∗ map] t ↦ s ∈ abs_hist, ⎡ know_frag_history_loc ℓ t s ⎤) ∗
+        "#physHist" ∷
+          ([∗ map] t ↦ msg ∈ phys_hist,
+             (* When we load a message for this location only the views in that
+              * message are physically added to our thread. If we want to access the
+              * invariants for all the prior messages then we need to remember that
+              * that these views have been added. We may however be able to lift this
+              * requirement to make [mapsto_at] flush free due to how predicates are
+              * used in [wp_load_at] (only objective things can be extracted). *)
+             have_msg_store_view msg ∗
+             ⎡ know_phys_hist_msg ℓ t msg ⎤) ∗
+        "#offset" ∷ ⎡ offset_loc ℓ offset ⎤ ∗
+        "#tSLe" ∷ have_SV ℓ (tS - offset)).
+
+  (*** Lower-bound assertions *)
+  Definition lb_base ℓ prot offset tS (s : ST) : dProp Σ :=
+    "#locationProtocol" ∷ ⎡ know_protocol ℓ prot ⎤ ∗
+    "#knowFragHist" ∷ ⎡ know_frag_history_loc ℓ tS s ⎤ ∗
+    "#offset" ∷ ⎡ offset_loc ℓ offset ⎤ ∗
+    "#tSLe" ∷ have_SV ℓ (tS - offset).
+
+  Definition store_lb ℓ prot (s : ST) : dProp Σ :=
+    ∃ (tS : nat) (offset : nat),
+      "#lbBase" ∷ lb_base ℓ prot offset tS s.
+
+  Definition flush_lb ℓ prot (s : ST) : dProp Σ :=
+    ∃ (tF : nat) offset,
+      "#lbBase" ∷ lb_base ℓ prot offset tF s ∗
+      (* Either we have something in the flush view or the location is
+      persisted. The later case is for after a crash where we don't have
+      anything in the flush view. *)
+      "#viewFact" ∷ (have_FV_strong ℓ (tF - offset) ∨
+                    ⎡ persisted_loc ℓ (tF - offset) ⎤).
+
+  Definition persist_lb ℓ prot (sP : ST) : dProp Σ :=
+    ∃ tP offset,
+      "#lbBase" ∷ lb_base ℓ prot offset tP sP ∗
+      (* We have the persisted state in our store view. *)
+      "#tPLe" ∷ have_FV ℓ (tP - offset) ∗
+      "persisted" ∷ ⎡ persisted_loc ℓ (tP - offset) ⎤.
+
+  Program Definition seen_view msg : dProp Σ :=
+    MonPred (λ TV,
+      ⌜ msg.(msg_store_view) ⊑ (store_view TV) ⌝
+      ∗
+      ⌜ msg.(msg_persisted_after_view) ⊑ (flush_view TV) ⌝
+    )%I _.
+  Next Obligation. solve_proper. Qed.
+
+  Definition seen_state ℓ (s : ST) : dProp Σ :=
+    ∃ (t offset : nat) (msg: message),
+      "#knowFragHist" ∷ ⎡ know_frag_history_loc ℓ t s ⎤ ∗
+      "#offset" ∷ ⎡ offset_loc ℓ offset ⎤ ∗
+      "#tSLe" ∷ have_SV ℓ (t - offset) ∗
+      "#knowPhysMsg" ∷ ⎡ know_phys_hist_msg ℓ t msg ⎤ ∗
+      "#seenView" ∷ seen_view msg.
+
+  Definition seen_state_post_fence ℓ (s : ST) : dProp Σ :=
+    ∃ (t offset : nat) (msg: message),
+      "#knowFragHist" ∷ ⎡ know_frag_history_loc ℓ t s ⎤ ∗
+      "#offset" ∷ ⎡ offset_loc ℓ offset ⎤ ∗
+      "#tSLe" ∷ have_SV ℓ (t - offset) ∗
+      "#knowPhysMsg" ∷ ⎡ know_phys_hist_msg ℓ t msg ⎤ ∗
+      "#haveMsg" ∷ have_msg_post_fence msg.
+
+  #[global] Instance seen_view_buffer_free msg:
+    BufferFree (seen_view msg).
+  Proof. rewrite /IntoNoBuffer. iModel. done. Qed.
+
+  #[global] Instance seen_view_persistent msg:
+    Persistent (seen_view msg).
+  Proof. rewrite /Persistent. iModel. iIntros "% !>". done. Qed.
+
+  Lemma seen_view_have_msg_post_fence msg:
+    seen_view msg -∗ have_msg_post_fence msg.
+  Proof.
+    iModel.
+    iIntros "[% %]".
+    simpl.
+    iSplit; iPureIntro; first done.
+    solve_view_le.
+  Qed.
+
+  (*** Crash assertions. *)
+  Definition crashed_in prot ℓ σ : dProp Σ :=
+    "#persistLb" ∷ persist_lb ℓ prot (prot.(p_bumper) σ) ∗
+    "#crashedIn" ∷ ⎡ crashed_in_loc ℓ σ ⎤.
+
+  (* [ℓ] was not recovered at the last crash. *)
+  Definition lost ℓ : dProp Σ :=
+    ∃ OCV,
+      "#crashed" ∷ ⎡ crashed_at_offset OCV ⎤ ∗
+      "%notInCV" ∷ ⌜ℓ ∉ dom OCV⌝.
+
+  (*** Combo assertions. *)
+  #[local] Notation "l ↦_{ prot }^{ q } ss" := (mapsto_na l prot q ss) (at level 20).
+  Definition mapsto_na_flushed ℓ prot q (σ: ST) : dProp Σ :=
+  ∃ (σs : list ST),
+    "%lastEq" ∷ ⌜ list.last σs = Some σ ⌝ ∗
+    "pts" ∷ ℓ ↦_{prot}^{q} σs ∗
+    "#flushLb" ∷ flush_lb ℓ prot σ.
+End location_assertions.
+
+(** Notation for the exclusive points-to predicate. *)
+Notation "l ↦_{ prot } ss" := (mapsto_na l prot 1 ss) (at level 20).
+Notation "l ↦_{ prot }^{ q } ss" := (mapsto_na l prot q ss) (at level 20).
+(* Notation "l ↦^{ p } ss" := (mapsto_na p l 1 ss) (at level 20). *)
+(* Notation "l ↦ ss" := (mapsto_na false l 1 ss) (at level 20). *)
+(* Notation "l ↦{ q } ss" := (mapsto_na false l q ss) (at level 20). *)
+(* Notation "l ↦ₚ ss" := (mapsto_na true l 1 ss) (at level 20). *)
+(* Notation "l ↦ₚ{ q } ss" := (mapsto_na true l q ss) (at level 20). *)
+(* Notation "l ↦ xs ; ys | P" := (mapsto_na l xs ys P) (at level 20). *)
+
+(** Notation for the shared points-to predicate. *)
+(* Notation "l ↦ ( s1 , s2 , s3 )  | P" := (mapsto_shared l s1 s2 s3 P) (at level 20). *)
+Notation "l ↦_AT^{ prot } ss" := (mapsto_at l prot ss) (at level 20).
