src/high/protocol_defs.v
@@ -1,0 +1,122 @@
+From iris.proofmode Require Import proofmode.
+From iris_named_props Require Import named_props.
+
+From self Require Import encode_relation.
+
+From self.high Require Import dprop generational_resources modalities monpred_simpl predicates.
+From self.high.lib Require Import abstract_state.
+
+From self.lang Require Import lang.
+
+(* A handy alias for the type of location predicates. *)
+Definition loc_pred `{nvmHighGS} ST `{AbstractState ST} := ST → val → dProp Σ.
+
+Definition loc_predO `{nvmHighGS} ST := ST -d> val -d> dPropO Σ.
+
+(* A protocol consists of
+  - A predicate [p_inv] that holds for each write and corresponding state of the
+    location.
+  - A function [bumper] that specifies how the state of a location changes
+    after a crash. *)
+
+Record LocationProtocol ST `{AbstractState ST, nvmHighGS} := MkProt {
+  p_full : loc_pred ST;
+  p_read : loc_pred ST;
+  p_pers : loc_pred ST;
+  p_bumper : ST → ST;
+}.
+
+#[global] Arguments MkProt   {ST _ _ _ _ _ _ _} _%_I _%_I _%_I _.
+#[global] Arguments p_full   {ST _ _ _ _ _ _ _} _.
+#[global] Arguments p_read   {ST _ _ _ _ _ _ _} _.
+#[global] Arguments p_pers   {ST _ _ _ _ _ _ _} _.
+#[global] Arguments p_bumper {ST _ _ _ _ _ _ _} _ _.
+
+(** [know_protocol] represents the knowledge that a location is associated with a
+specific protocol. It's defined simply using more "primitive" assertions. *)
+Definition know_protocol `{AbstractState ST, nvmHighGS}
+           ℓ (prot : LocationProtocol ST) : iProp Σ :=
+  "#knowFullPred" ∷  know_full_pred ℓ prot.(p_full)  ∗
+  "#knowReadPred" ∷  know_read_pred ℓ prot.(p_read)  ∗
+  "#knowPersPred" ∷  know_pers_pred ℓ prot.(p_pers)  ∗
+  "#knowPreorder" ∷  know_preorder_loc ℓ (⊑@{ST})  ∗
+  "#knowBumper" ∷  know_bumper ℓ prot.(p_bumper) .
+
+Section encoded.
+  #[local] Existing Instance nvmHighGS_inG.
+  Definition know_protocol_enc `{nvmHighGS} ℓ
+    (encp_full encp_read encp_pers : (enc_predicateO))
+    (order : extra.relation2 positive) (bump : positive → option positive) : iProp Σ :=
+    know_pred_ra full_predicates_name ℓ (unwrapped_pred_to_ra (encoded_pred_unwrap encp_full)) ∗
+    know_pred_ra read_predicates_name ℓ (unwrapped_pred_to_ra (encoded_pred_unwrap encp_read)) ∗
+    know_pred_ra pers_predicates_name ℓ (unwrapped_pred_to_ra (encoded_pred_unwrap encp_pers)) ∗
+    (ℓ ↪[preorders_name, drop_OCV]□ order) ∗
+    (ℓ ↪[bumpers_name, drop_OCV]□ bump).
+End encoded.
+
+Lemma encode_bumper_bump_mono `{AbstractState ST}
+      (bumper : ST → ST) `{!Proper ((⊑@{ST}) ==> (⊑))%signature bumper}
+      (x y x' y' : positive) :
+  encode_bumper bumper x = Some x' →
+  encode_bumper bumper y = Some y' →
+  encode_relation (⊑@{ST}) x y →
+  encode_relation (⊑@{ST}) x' y'.
+Proof.
+  rewrite /encode_bumper. rewrite /encode_relation.
+  intros (sx & -> & <-)%encode_bumper_Some_decode.
+  intros (sy & -> & <-)%encode_bumper_Some_decode.
+  rewrite !decode_encode /=.
+  solve_proper.
+Qed.
+
+Section protocol.
+  Context `{nvmHighGS, AbstractState ST}.
+
+  Implicit Types (prot : LocationProtocol ST).
+
+  #[local] Existing Instance nvmHighGS_inG.
+  #[local] Existing Instance nvmHighGpreS_bumpers.
+
+  Lemma nextgen_know_protocol ℓ prot :
+    know_protocol ℓ prot -∗
+    ⚡==> base_if_rec ℓ (lastgen_know_bumper ℓ prot.(p_bumper) ∗ lastgen_know_preorder_loc ℓ (⊑@{ST}) ∗ know_protocol ℓ prot).
+  Proof.
+    iNamed 1.
+    iPoseProof (ghost_map_elem_into_nextgen_ifrec with "knowPreorder") as "knowPreorder'".
+    iPoseProof (ghost_map_elem_into_nextgen_ifrec with "[]") as "knowBumper'".
+    { iDestruct "knowBumper" as "[? $]". }
+    iDestruct "knowBumper" as "[% _]".
+    iModIntro.
+    iDestruct "knowBumper'" as "[$ knowBumper']".
+    iDestruct "knowPreorder'" as "[$ knowPreorder']".
+    rewrite -?if_rec_lift_if_rec.
+
+    iModIntro. iFrame "#%".
+  Qed.
+
+  #[global] Instance know_protocol_into_nextgen ℓ prot :
+    base_IntoNextgen
+      ( know_protocol ℓ prot )
+      (base_if_rec ℓ (lastgen_know_bumper ℓ prot.(p_bumper) ∗ lastgen_know_preorder_loc ℓ (⊑@{ST}) ∗ know_protocol ℓ prot )).
+  Proof.
+    rewrite /base_IntoNextgen.
+    iIntros "P".
+    by iApply nextgen_know_protocol.
+  Qed.
+
+  #[global] Instance know_protocol_contractive ℓ bumper :
+    Contractive (λ (invs : (prodO (prodO (loc_predO ST) (loc_predO ST)) (loc_predO ST))),
+                      let '(full, read, pers) := invs in
+                      (know_protocol ℓ (MkProt full read pers bumper))).
+  Proof.
+    rewrite /know_protocol.
+    intros ????.
+    destruct x as [[full read] pers].
+    destruct y as [[full' read'] pers'].
+    simpl.
+    repeat
+      (done ||
+       f_contractive ||
+       f_equiv); apply H2.
+  Qed.
+End protocol.
